crypto/ec/Hacl.EC.Curve25519.Bignum.Fproduct.Lemmas.fst
@@ -4,18 +4,15 @@ open FStar.Mul
 open FStar.ST
 open FStar.HyperStack
 open FStar.Ghost
-open Hacl.UInt64
-open Hacl.SBuffer
+open FStar.Buffer
 open FStar.Math.Lib
+open FStar.Math.Lemmas
+
+open Hacl.UInt64
+
 open Hacl.EC.Curve25519.Parameters
 open Hacl.EC.Curve25519.Bigint
-
-
-#reset-options "--initial_fuel 0 --max_fuel 0"
-
-(* Module abbreviations *)
-module HH = FStar.HyperHeap
-module HS = FStar.HyperStack
+open Hacl.EC.Curve25519.Bignum.Lemmas.Utils
 
 module U8  = FStar.UInt8
 module U32 = FStar.UInt32
@@ -23,927 +20,419 @@ module H8  = Hacl.UInt8
 module H32  = Hacl.UInt32
 module H64  = Hacl.UInt64
 
-(* Lemma : additivity property of the "bitweight" function if the template is normalized *)
-val bitweight_lemma_1: t:template{forall (n:nat). t n = t 0} -> i:nat -> Lemma (bitweight t i = i * (t 0))
-let rec bitweight_lemma_1 t i = 
-  admit(); // OK
-  match i with
-  | 0 -> ()
-  | _ -> 
-    (* FproductLemmas.auxiliary_lemma_2 i; *)
-    assert(t (i-1) = t 0); 
-    assert(bitweight t i = t 0 + bitweight t (i-1));
-    bitweight_lemma_1 t (i-1)
-    (* FproductLemmas.auxiliary_lemma_3 (t 0) i *)
 
-val bitweight_lemma_0: t:template{ forall (n:nat). t n = t 0 } -> i:nat -> j:nat -> 
-  Lemma ( bitweight t (i+j) = bitweight t i + bitweight t j)
-let rec bitweight_lemma_0 t i j =
-  admit(); // OK
-  bitweight_lemma_1 t (i+j); 
-  bitweight_lemma_1 t i; bitweight_lemma_1 t j
-  (* FproductLemmas.auxiliary_lemma_4 (t 0) i j *)
+#reset-options "--z3timeout 20 --initial_fuel 0 --max_fuel 0"
 
-(* Lemma : combines the additivity property of the bitweight function and the exponential property 
-   of the pow2 function *)
-val auxiliary_lemma_1: 
-  t:template{ forall (n:nat). t n = t 0 } -> a:nat -> b:nat -> 
-  Lemma (ensures (pow2 (bitweight t (a+b)) = pow2 (bitweight t a) * pow2 (bitweight t b)))
-let auxiliary_lemma_1 t a b =
-  admit(); // OK
-  bitweight_lemma_0 t a b;
-  Math.Lemmas.pow2_exp_1 (bitweight t a) (bitweight t b)
+let isMultiplication (h0:mem) (h1:mem) (a:bigint) (b:bigint) (c:bigint_wide) : GTot Type0 =
+  live h0 a /\ live h0 b /\ live h1 c
+  /\ length c >= 2*norm_length-1
+  /\ (
+    let a0 = v (get h0 a 0) in let a1 = v (get h0 a 1) in let a2 = v (get h0 a 2) in
+    let a3 = v (get h0 a 3) in let a4 = v (get h0 a 4) in let b0 = v (get h0 b 0) in
+    let b1 = v (get h0 b 1) in let b2 = v (get h0 b 2) in let b3 = v (get h0 b 3) in
+    let b4 = v (get h0 b 4) in 
+    let open Hacl.UInt128 in
+    let c0 = v (get h1 c 0) in let c1 = v (get h1 c 1) in
+    let c2 = v (get h1 c 2) in let c3 = v (get h1 c 3) in let c4 = v (get h1 c 4) in
+    let c5 = v (get h1 c 5) in let c6 = v (get h1 c 6) in let c7 = v (get h1 c 7) in
+    let c8 = v (get h1 c 8) in
+    ( c0 = a0 * b0
+      /\ c1 = a0 * b1 + a1 * b0
+      /\ c2 = a0 * b2 + a1 * b1 + a2 * b0
+      /\ c3 = a0 * b3 + a1 * b2 + a2 * b1 + a3 * b0
+      /\ c4 = a0 * b4 + a1 * b3 + a2 * b2 + a3 * b1 + a4 * b0
+      /\ c5 = a1 * b4 + a2 * b3 + a3 * b2 + a4 * b1
+      /\ c6 = a2 * b4 + a3 * b3 + a4 * b2
+      /\ c7 = a3 * b4 + a4 * b3
+      /\ c8 = a4 * b4 ) )
 
-abstract type partialEquality (ha:heap) (a:bigint_wide{live ha a})
-			    (hb:heap) (b:bigint_wide{live hb b}) 
-			    (len:nat{len <= length a /\ len <= length b}) =
-  (forall (i:nat). {:pattern (v (get ha a i))}
-    i < len ==> v (get ha a i) = v (get hb b i))
+let isMultiplication_
+  (h1:mem)
+  (a0:int) (a1:int) (a2:int) (a3:int) (a4:int)
+  (b0:int) (b1:int) (b2:int) (b3:int) (b4:int)
+  (c:bigint_wide) : GTot Type0 =
+  live h1 c /\ length c >= 2*norm_length-1
+  /\ ( let open Hacl.UInt128 in
+      let c0 = v (get h1 c 0) in let c1 = v (get h1 c 1) in
+      let c2 = v (get h1 c 2) in let c3 = v (get h1 c 3) in let c4 = v (get h1 c 4) in
+      let c5 = v (get h1 c 5) in let c6 = v (get h1 c 6) in let c7 = v (get h1 c 7) in
+      let c8 = v (get h1 c 8) in
+      ( c0 = a0 * b0
+	/\ c1 = a0 * b1 + a1 * b0
+	/\ c2 = a0 * b2 + a1 * b1 + a2 * b0
+	/\ c3 = a0 * b3 + a1 * b2 + a2 * b1 + a3 * b0
+	/\ c4 = a0 * b4 + a1 * b3 + a2 * b2 + a3 * b1 + a4 * b0
+	/\ c5 = a1 * b4 + a2 * b3 + a3 * b2 + a4 * b1
+	/\ c6 = a2 * b4 + a3 * b3 + a4 * b2
+	/\ c7 = a3 * b4 + a4 * b3
+	/\ c8 = a4 * b4 ) )
 
-abstract type storesSum (hc:heap) (c:bigint_wide{live hc c})
-		      (ha:heap) (a:bigint_wide{live ha a})
-		      (hb:heap) (b:bigint_wide{live hb b})
-		      (a_idx:nat)
-		      (len:nat{a_idx+len <= length a /\ len <= length b /\ a_idx+len <= length c}) =
- (forall (i:nat). {:pattern (v (get hc c (i+a_idx)))}
-   (i < len ==> v (get hc c (i+a_idx)) = v (get ha a (i+a_idx)) + v (get hb b i)))
-			      
-val multiplication_step_lemma_1: h0:heap -> h1:heap -> a:bigint_wide{live h0 a} -> 
-  b:bigint_wide{live h0 b} -> c:bigint_wide{live h1 c} ->
-  idx:nat -> len:pos{len+idx <= length a /\ len <= length b /\ length a = length c } -> Lemma
-    (requires (
-      storesSum h1 c h0 a h0 b idx len
-      /\ partialEquality h1 c h0 a idx
-      /\ eval_wide h1 c (len-1+idx) = eval_wide h0 a (len-1+idx) + pow2 (bitweight (templ) idx) * eval_wide h0 b (len-1)))
-    (ensures (eval_wide h1 c (len+idx) = eval_wide h0 a (len+idx) +  
-		          pow2 (bitweight (templ) idx) * eval_wide h0 b (len-1)  +	        
-			  pow2 (bitweight (templ) (len-1+idx)) * v (get h0 b (len-1))))
-let multiplication_step_lemma_1 h0 h1 a b c idx len = ()
-  (* admit(); // OK *)
-  (* let t = templ in *)
-  (* (\* FproductLemmas.auxiliary_lemma_0 len idx 1;  *\) *)
-  (* eval_wide_def h1 c (len+idx);  *)
-  (* (\* FproductLemmas.auxiliary_lemma_00 len idx 1;    *\) *)
-  (* cut (v (get h1 c (len+idx-1)) = v (get h0 a (len+idx-1)) + v (get h0 b (len-1)) /\ True);  *)
-  (* cut (True /\ eval h1 c (len+idx) = pow2 (bitweight t (len+idx-1)) * v (get h1 c (len+idx-1)) + eval h1 c (len+idx-1));  *)
-  (* cut (eval h1 c (len+idx) = eval h1 c (len+idx-1) + pow2 (bitweight t (len+idx-1)) * v (get h1 c (len+idx-1)) /\ True ); *)
-  (* cut (eval h1 c (len+idx-1) = eval h0 a (len+idx-1) + (pow2 (bitweight t idx)) * eval h0 b (len-1) /\ True);  *)
-  (* cut (v (get h1 c (len+idx-1)) = v (get h0 a (len+idx-1)) + v (get h0 b (len-1)) /\ True);  *)
-  (* cut (eval h1 c (len+idx) =  *)
-  (* 	(eval h0 a (len+idx-1) + (pow2 (bitweight t idx)) * eval h0 b (len-1)) *)
-  (* 	+ pow2 (bitweight t (len-1+idx)) * (v (get h0 a (len+idx-1)) + v (get h0 b (len-1))) /\ True);  *)
-  (* Math.Axioms.distributivity_add_right (pow2 (bitweight t (len-1+idx))) (v (get h0 a (len+idx-1))) (v (get h0 b (len-1)));  *)
-  (* cut (True /\ eval h1 c (len+idx) =  *)
-  (* 	(eval h0 a (len+idx-1) + (pow2 (bitweight t idx)) * eval h0 b (len-1)) *)
-  (* 	+ (pow2 (bitweight t (len-1+idx)) * v (get h0 a (len+idx-1)) *)
-  (*       + pow2 (bitweight t (len-1+idx)) * v (get h0 b (len-1))));  *)
-  (* (\* FproductLemmas.remove_paren_lemma (eval h0 a (len+idx-1)) ((pow2 (bitweight t idx)) * eval h0 b (len-1)) ((pow2 (bitweight t (len-1+idx)) * v (get h0 a (len+idx-1)) + pow2 (bitweight t (len-1+idx)) * v (get h0 b (len-1))));  *\) *)
-  (* cut (True /\ eval h1 c (len+idx) =  *)
-  (* 	eval h0 a (len+idx-1) + (pow2 (bitweight t idx)) * eval h0 b (len-1) *)
-  (* 	+ (pow2 (bitweight t (len-1+idx)) * v (get h0 a (len+idx-1)) *)
-  (*       + pow2 (bitweight t (len-1+idx)) * v (get h0 b (len-1)))); *)
-  (* (\* FproductLemmas.remove_paren_lemma (eval h0 a (len+idx-1) + (pow2 (bitweight t idx)) * eval h0 b (len-1))  *\) *)
-  (* (\* 		     (pow2 (bitweight t (len-1+idx)) * v (get h0 a (len+idx-1))) *\) *)
-  (* (\* 		     (pow2 (bitweight t (len-1+idx)) * v (get h0 b (len-1)));  *\) *)
-  (* cut (True /\ eval h1 c (len+idx) =  *)
-  (* 	eval h0 a (len+idx-1) + pow2 (bitweight t idx) * eval h0 b (len-1)  + *)
-  (* 	pow2 (bitweight t (len-1+idx)) * v (get h0 a (len+idx-1)) +    	         *)
-  (*         pow2 (bitweight t (len-1+idx)) * v (get h0 b (len-1)));  *)
-  (* (\* FproductLemmas.auxiliary_lemma_6 (eval h0 a (len+idx-1))  *\) *)
-  (* (\* 				  (pow2 (bitweight t idx) * eval h0 b (len-1)) *\) *)
-  (* (\* 				  (pow2 (bitweight t (len-1+idx)) * v (get h0 a (len+idx-1)))     *\) *)
-  (* (\* 				  (pow2 (bitweight t (len-1+idx)) * v (get h0 b (len-1))); *\) *)
-  (* cut (True /\ eval h1 c (len+idx) =  *)
-  (* 	pow2 (bitweight t (len-1+idx)) * v (get h0 a (len+idx-1)) + eval h0 a (len+idx-1) +  *)
-  (*         pow2 (bitweight t idx) * eval h0 b (len-1)  +	         *)
-  (*         pow2 (bitweight t (len-1+idx)) * v (get h0 b (len-1)));  *)
-  (* eval_wide_def h0 a (len+idx); *)
-  (* cut (True /\ eval h0 a (len+idx) = pow2 (bitweight t (len+idx-1)) * v (get h0 a (len+idx-1)) + eval h0 a (len+idx-1));  *)
-  (* cut (True /\ eval h1 c (len+idx) =  *)
-  (* 		eval h0 a (len+idx)  *)
-  (* 		+ pow2 (bitweight t idx) * eval h0 b (len-1)   *)
-  (* 		+ pow2 (bitweight t (len-1+idx)) * v (get h0 b (len-1))) *)
 
-(* #reset-options *)
+#reset-options "--z3timeout 20 --initial_fuel 0 --max_fuel 0"
 
-(* Lemma : second half of the helper for the multiplication_step_lemma *)
-val multiplication_step_lemma_2: h0:heap -> h1:heap -> a:bigint_wide{live h0 a } -> 
-  b:bigint_wide{live h0 b} -> c:bigint_wide{live h1 c} -> idx:nat ->
-  len:pos{len+idx <= length a /\ len <= length b /\ length a = length c} -> Lemma 
-    (requires (
-	 eval_wide h1 c (len+idx) = eval_wide h0 a (len+idx) +  
-                          pow2 (bitweight (templ) idx) * eval_wide h0 b (len-1)  +	        
-			  pow2 (bitweight (templ) (len-1+idx)) * v (get h0 b (len-1))
-    ))
-    (ensures (eval_wide h1 c (len+idx) = eval_wide h0 a (len+idx) + pow2 (bitweight (templ) idx) * eval_wide h0 b len))
-let multiplication_step_lemma_2 h0 h1 a b c idx len = 
-  admit(); // OK
-  (* FproductLemmas.auxiliary_lemma_0 len idx 1; *)
-  auxiliary_lemma_1 (templ) idx (len-1); 
-  (* FproductLemmas.auxiliary_lemma_00 len (-1) idx; *)
-  (* FproductLemmas.auxiliary_lemma_01 (len-1) idx;  *)
-  cut (True /\ pow2 (bitweight (templ) (len-1+idx)) = pow2 (bitweight (templ) idx) * pow2 (bitweight (templ) (len-1)) ); 
-  Math.Axioms.paren_mul_left (pow2 (bitweight (templ) idx)) (pow2 (bitweight (templ) (len-1))) (v (get h0 b (len-1))); 
-  cut (eval_wide h1 c (len+idx) = eval_wide h0 a (len+idx) 
-			     + pow2 (bitweight (templ) idx) * eval_wide h0 b (len-1)
-			     + pow2 (bitweight (templ) idx) * pow2 (bitweight (templ) (len-1)) * v (get h0 b (len-1)) /\ True); 
-  Math.Axioms.distributivity_add_right (pow2 (bitweight (templ) idx)) (eval_wide h0 b (len-1)) (pow2 (bitweight (templ) (len-1)) * v (get h0 b (len-1)));  
-  eval_wide_def h0 b len; 
-  cut (True /\ eval_wide h0 b len = eval_wide h0 b (len-1) + (pow2 (bitweight (templ) (len-1))) * v (get h0 b (len-1)) );  
-  cut (True /\ pow2 (bitweight (templ) (len-1+idx)) * v (get h0 b (len-1)) =
-        pow2 (bitweight (templ) idx) * pow2 (bitweight (templ) (len-1)) * v (get h0 b (len-1))); 
-  cut ( True /\ eval_wide h1 c (len+idx) = eval_wide h0 a (len+idx) + pow2 (bitweight (templ) idx) * eval_wide h0 b len) 
+val lemma_multiplication_0:
+  a0:H64.t -> a1:H64.t -> a2:H64.t -> a3:H64.t -> a4:H64.t ->
+  b0:H64.t -> b1:H64.t -> b2:H64.t -> b3:H64.t -> b4:H64.t ->
+  Lemma (requires (
+	  v a0 < pow2 51 /\ v a1 < pow2 51 /\ v a2 < pow2 51 /\ v a3 < pow2 51 /\ v a4 < pow2 51
+	  /\ v b0 < pow2 51 /\ v b1 < pow2 51 /\ v b2 < pow2 51 /\ v b3 < pow2 51 /\ v b4 < pow2 51))
+	(ensures  (
+	  v a0 * v b0 < pow2 128 /\ v a1 * v b0 < pow2 128 /\ v a2 * v b0 < pow2 128
+	  /\ v a3 * v b0 < pow2 128 /\ v a4 * v b0 < pow2 128 /\ v a0 * v b1 < pow2 128
+	  /\ v a1 * v b1 < pow2 128 /\ v a2 * v b1 < pow2 128 /\ v a3 * v b1 < pow2 128
+	  /\ v a4 * v b1 < pow2 128 /\ v a0 * v b2 < pow2 128 /\ v a1 * v b2 < pow2 128
+	  /\ v a2 * v b2 < pow2 128 /\ v a3 * v b2 < pow2 128 /\ v a4 * v b2 < pow2 128
+	  /\ v a0 * v b3 < pow2 128 /\ v a1 * v b3 < pow2 128 /\ v a2 * v b3 < pow2 128
+	  /\ v a3 * v b3 < pow2 128 /\ v a4 * v b3 < pow2 128 /\ v a0 * v b4 < pow2 128
+	  /\ v a1 * v b4 < pow2 128 /\ v a2 * v b4 < pow2 128 /\ v a3 * v b4 < pow2 128
+	  /\ v a4 * v b4 < pow2 128
+	  /\ v a0 * v b1 + v a1 * v b0 < pow2 128
+	  /\ v a0 * v b2 + v a1 * v b1 < pow2 128
+	  /\ v a0 * v b2 + v a1 * v b1 + v a2 * v b0 < pow2 128
+	  /\ v a0 * v b3 + v a1 * v b2 < pow2 128
+	  /\ v a0 * v b3 + v a1 * v b2 + v a2 * v b1 < pow2 128
+	  /\ v a0 * v b3 + v a1 * v b2 + v a2 * v b1 + v a3 * v b0 < pow2 128
+	  /\ v a0 * v b4 + v a1 * v b3 < pow2 128
+	  /\ v a0 * v b4 + v a1 * v b3 + v a2 * v b2 < pow2 128
+	  /\ v a0 * v b4 + v a1 * v b3 + v a2 * v b2 + v a3 * v b1 < pow2 128
+	  /\ v a0 * v b4 + v a1 * v b3 + v a2 * v b2 + v a3 * v b1 + v a4 * v b0 < pow2 128
+	  /\ v a1 * v b4 + v a2 * v b3 < pow2 128
+	  /\ v a1 * v b4 + v a2 * v b3 + v a3 * v b2 < pow2 128
+	  /\ v a1 * v b4 + v a2 * v b3 + v a3 * v b2 + v a4 * v b1 < pow2 128
+	  /\ v a2 * v b4 + v a3 * v b3 < pow2 128
+	  /\ v a2 * v b4 + v a3 * v b3 + v a4 * v b2 < pow2 128
+	  /\ v a3 * v b4 + v a4 * v b3 < pow2 128
+	  ))
+let lemma_multiplication_0 a0 a1 a2 a3 a4 b0 b1 b2 b3 b4 =
+  assert(forall (a:nat) (b:nat) c d. {:pattern (a * b); (c * d)} (a < c /\ b < d) ==> a * b < c * d);
+  pow2_plus 51 51;
+  pow2_lt_compat 128 102;
+  pow2_double_sum 102;
+  pow2_lt_compat 128 102;
+  pow2_double_sum 103;
+  pow2_lt_compat 128 104;
+  pow2_double_sum 104;
+  pow2_lt_compat 128 105
 
-(* #reset-options *)
 
-(* Lemma : changes the result of the addition function into the equivalent relation between 
-  evaluated bigints *)
-val multiplication_step_lemma: h0:heap -> h1:heap -> a:bigint_wide{live h0 a } -> 
-  b:bigint_wide{live h0 b} -> c:bigint_wide{live h1 c} -> idx:nat ->
-  len:nat{len+idx <= length a /\ len <= length b /\ length a = length c} -> Lemma
-    (requires (storesSum h1 c h0 a h0 b idx len /\ partialEquality h1 c h0 a idx))
-    (ensures (eval_wide h1 c (len+idx) = eval_wide h0 a (len+idx) + pow2 (bitweight (templ) idx) * eval_wide h0 b len
-    ))
-let rec multiplication_step_lemma h0 h1 a b c idx len =
-  admit(); // OK
-  match len with
-  | 0 ->
-    cut (forall (i:nat). i < idx ==> v (get h1 c i) = v (get h0 a i)); 
-    (* eval_eq_lemma h0 h1 a c idx;  *)
-    (* FproductLemmas.auxiliary_lemma_02 len idx; *)
-    cut (True /\ len+idx = idx); 
-    cut (True /\ eval_wide h0 b len = 0);
-    (* FproductLemmas.auxiliary_lemma_03 (pow2 (bitweight (templ) idx)); *)
-    cut (True /\ pow2 (bitweight (templ) idx) * 0 = 0);
-    cut (True /\ eval_wide h1 c (len+idx) = eval_wide h0 a (len+idx))
-  | _ ->   
-     (* FproductLemmas.auxiliary_lemma_0 len idx 1;  *)
-     (* FproductLemmas.auxiliary_lemma_2 len; *)
-     multiplication_step_lemma h0 h1 a b c idx (len-1); 
-     multiplication_step_lemma_1 h0 h1 a b c idx len; 
-     multiplication_step_lemma_2 h0 h1 a b c idx len
+#reset-options "--z3timeout 20 --initial_fuel 0 --max_fuel 0"
 
-(* #reset-options *)
+let u51 = x:Hacl.UInt64.t{v x < pow2 51}
 
-let (max_limb:nat) = parameters_lemma_1 (); (platform_wide - log_2 norm_length - 1) / 2
-let (max_wide:nat) = 2 * max_limb
 
-abstract type fitsMaxLimbSize (h:heap) (a:bigint{live h a}) =
-  (forall (i:nat). {:pattern (S64.v (get h a i))} i < norm_length ==> S64.v (get h a i) < pow2 max_limb)
-  
-(* Lemma *)
-val auxiliary_lemma_2: h0:heap -> h1:heap -> h2:heap -> a:bigint{live h0 a /\ fitsMaxLimbSize h0 a } ->
-  b:bigint{live h1 b /\ (forall (i:nat). i < norm_length ==> S64.v (get h1 b i) < pow2 max_limb)} ->
-  ctr:nat{(ctr <= norm_length)} -> c:bigint{live h2 c /\ maxValue h2 c (length c) <= ctr * (maxValueNorm h0 a * maxValueNorm h1 b)} -> Lemma ((maxValueNorm h0 a <= pow2 max_limb) /\ (maxValueNorm h1 b <= pow2 max_limb))
-let auxiliary_lemma_2 h0 h1 h2 a b ctr c = 
-  admit(); // OK
-  ()
+let lemma_multiplication00 a b c :
+  Lemma (a * (b + c) = a * b + a * c)
+  = ()
+let lemma_multiplication01 a b c d:
+  Lemma (a * (b + c + d) = a * b + a * c + a * d)
+  = ()
+let lemma_multiplication02 a b c d e :
+  Lemma (a * (b + c + d + e) = a * b + a * c + a * d + a * e)
+  = ()
+let lemma_multiplication03 a b c d e f :
+  Lemma (a * (b + c + d + e + f) = a * b + a * c + a * d + a * e + a * f)
+  = ()
+private let lemma_multiplication03bis a b c d e f :
+  Lemma ((b + c + d + e + f) * a = b * a + c * a + d * a + e * a + f * a)
+  = ()
+private let lemma_multiplication04 a0 a1 a2 a3 a4 b0 b1 b2 b3 b4 :
+  Lemma ((a0+a1+a2+a3+a4)*(b0+b1+b2+b3+b4)
+    = a0*b0+a0*b1+a0*b2+a0*b3+a0*b4
+      +a1*b0+a1*b1+a1*b2+a1*b3+a1*b4
+      +a2*b0+a2*b1+a2*b2+a2*b3+a2*b4
+      +a3*b0+a3*b1+a3*b2+a3*b3+a3*b4
+      +a4*b0+a4*b1+a4*b2+a4*b3+a4*b4)
+  = lemma_multiplication03bis (b0+b1+b2+b3+b4) a0 a1 a2 a3 a4;
+    lemma_multiplication03 a0 b0 b1 b2 b3 b4;
+    lemma_multiplication03 a1 b0 b1 b2 b3 b4;
+    lemma_multiplication03 a2 b0 b1 b2 b3 b4;
+    lemma_multiplication03 a3 b0 b1 b2 b3 b4;
+    lemma_multiplication03 a4 b0 b1 b2 b3 b4
 
-(* #reset-options *)
+#reset-options "--z3timeout 5 --initial_fuel 0 --max_fuel 0"
 
-(* Lemma : bounds the maxValues product *)
-val auxiliary_lemma_3: h0:heap -> h1:heap -> h2:heap -> a:bigint{live h0 a /\ maxValueNorm h0 a <= pow2 max_limb} -> b:bigint{live h1 b /\ maxValueNorm h1 b <= pow2 max_limb} -> ctr:nat{ctr <= norm_length} ->
-  c:bigint_wide{live h2 c /\ maxValue_wide h2 c (length c) <= ctr * (maxValueNorm h0 a * maxValueNorm h1 b)} ->
-  Lemma (maxValueNorm h0 a * maxValueNorm h1 b <= pow2 max_wide)
-let auxiliary_lemma_3 h0 h1 h2 a b ctr c =
-  admit(); // OK
-  let s = max_wide in
-  Math.Axioms.slash_star_axiom max_limb 2 max_wide;
-  cut (max_limb = s / 2 /\ True); 
-  (* FproductLemmas.helper_lemma_3 (maxValueNorm h0 a) (maxValueNorm h1 b) (pow2 max_limb) (pow2 max_limb); *)
-  Math.Lemmas.pow2_exp_1 (s/2) (s/2); 
-  cut (maxValueNorm h0 a * maxValueNorm h1 b <= pow2 ((s/2)+(s/2)) /\ True); 
-  (* FproductLemmas.helper_lemma_2 (s/2); *)
-  Math.Lemmas.multiply_fractions s 2; 
-  cut ((s / 2)+(s/2) <= (s) /\ True);
-  if (((s/2)+(s/2)) < s ) then
-	Math.Lemmas.pow2_increases_1 s ((s/2)+(s/2));
-  cut (pow2 (((s/2)+(s/2))) <= pow2 s /\ True); 
-  cut (maxValueNorm h0 a * maxValueNorm h1 b <= pow2 s /\ True)
+let lemma_multiplication05
+  (a0:int) (a1:int) (a2:int) (a3:int) (a4:int)
+  (b0:int) (b1:int) (b2:int) (b3:int) (b4:int) :
+  Lemma ((a0 + pow2 51 * a1 + pow2 102 * a2 + pow2 153 * a3 + pow2 204 * a4)
+    * (b0 + pow2 51 * b1 + pow2 102 * b2 + pow2 153 * b3 + pow2 204 * b4)
+    = a0*b0+a0*(pow2 51*b1)+a0*(pow2 102*b2)+a0*(pow2 153*b3)+a0*(pow2 204*b4)
+      +(pow2 51*a1)*b0+(pow2 51*a1)*(pow2 51*b1)+(pow2 51*a1)*(pow2 102*b2)+(pow2 51*a1)*(pow2 153*b3)+(pow2 51*a1)*(pow2 204*b4)
+      +(pow2 102*a2)*b0+(pow2 102*a2)*(pow2 51*b1)+(pow2 102*a2)*(pow2 102*b2)+(pow2 102*a2)*(pow2 153*b3)+(pow2 102*a2)*(pow2 204*b4)
+      +(pow2 153*a3)*b0+(pow2 153*a3)*(pow2 51*b1)+(pow2 153*a3)*(pow2 102*b2)+(pow2 153*a3)*(pow2 153*b3)+(pow2 153*a3)*(pow2 204*b4)
+      +(pow2 204*a4)*b0+(pow2 204*a4)*(pow2 51*b1)+(pow2 204*a4)*(pow2 102*b2) +(pow2 204*a4)*(pow2 153*b3)+(pow2 204*a4)*(pow2 204*b4) )
+  = lemma_multiplication04 (a0) (pow2 51 * a1) (pow2 102 * a2) (pow2 153 * a3) (pow2 204 * a4)
+			   (b0) (pow2 51 * b1) (pow2 102 * b2) (pow2 153 * b3) (pow2 204 * b4)
 
-(* #reset-options *)
 
-abstract type partialEquality2 (ha:heap) (a:bigint_wide{live ha a})
-			       (hb:heap) (b:bigint_wide{live hb b}) 
-			       (len:nat)
-			       (len2:nat{len2 >= len /\ len2 <= length a /\ len2 <= length b}) =
-  (forall (i:nat). {:pattern (v (get ha a i))}
-    (i < len2 /\ i >= len) ==> v (get ha a i) = v (get hb b i))
+#reset-options "--z3timeout 20 --initial_fuel 0 --max_fuel 0"
 
-(* Lemma : extends the "eval" property to the total length if apporpriate *)
-val auxiliary_lemma_5: h0:heap -> h1:heap -> a:bigint_wide{live h0 a } -> b:bigint_wide{live h1 b} ->
-  c:int -> len:nat -> len2:nat{ len2 >= len /\ len2 <= length b /\ len2 <= length a } -> Lemma 
-    (requires ( (eval_wide h1 b len = eval_wide h0 a len + c)
-		/\ partialEquality2 h1 b h0 a len len2))
-    (ensures ( (eval_wide h1 b len2 = eval_wide h0 a len2 + c)))
-let rec auxiliary_lemma_5 h0 h1 a b c len len2 =
-  admit(); // OK
-  match len2 - len with
-  | 0 -> ()
-     (* FproductLemmas.auxiliary_lemma_8 len2 len *)
-  | _ ->
-     let t = templ in
-     (* FproductLemmas.auxiliary_lemma_7 len2 len; *)
-     auxiliary_lemma_5 h0 h1 a b c len (len2-1); 
-     cut (True /\ eval_wide h1 b (len2-1) = eval_wide h0 a (len2-1) + c); 
-     eval_wide_def h1 b len2; 
-     cut (True /\ eval_wide h1 b len2 = eval_wide h1 b (len2-1) + (pow2 (bitweight t (len2-1))) * v (get h1 b (len2-1))); 
-     cut (v (get h1 b (len2-1)) = v (get h0 a (len2-1)) /\ True); 
-     cut (True /\ eval_wide h1 b len2 = (eval_wide h0 a (len2-1) + c) + (pow2 (bitweight t (len2-1))) * v (get h0 a (len2-1))); 
-     (* FproductLemmas.auxiliary_lemma_04 (eval_wide h0 a (len2-1)) c ((pow2 (bitweight t (len2-1))) * v (get h0 a (len2-1)));   *)
-     eval_wide_def h0 a len2;
-     cut (True /\ eval_wide h1 b len2 = eval_wide h0 a len2 + c)
+private let lemma_multiplication060
+  (a0:int) (a1:int) (a2:int) (a3:int) (a4:int)
+  (b0:int) (b1:int) (b2:int) (b3:int) (b4:int) :
+  Lemma (
+    a0*b0+a0*(pow2 51*b1)+a0*(pow2 102*b2)+a0*(pow2 153*b3)+a0*(pow2 204*b4)
+    = a0 * b0 + pow2 51  * (a0 * b1) + pow2 102  * (a0 * b2) + pow2 153  * (a0 * b3) + pow2 204 * (a0 * b4) )
+  = ()
 
-(* #reset-options *)
+#reset-options "--z3timeout 20 --initial_fuel 0 --max_fuel 0"
 
-abstract type isScalarProduct 
-  (hc:heap) (c:bigint_wide{live hc c /\ length c >= norm_length})
-  (ha:heap) (a:bigint{live ha a /\ length a >= norm_length}) (s:s64) =
-    (forall (i:nat). {:pattern (v (get hc c i))}
-      (i<norm_length) ==> v (get hc c i) = S64.v (get ha a i) * S64.v s)  
-  
-val max_limb_lemma: a:nat -> b:nat -> 
-  Lemma
-    (requires (a < pow2 max_limb /\ b < pow2 max_limb))
-    (ensures (a * b < pow2 platform_wide))
-    [SMTPat (a * b)]
-let max_limb_lemma a b =
-  (* FproductLemmas.ineq_lemma_3 a b (pow2 max_limb); *)
-  Math.Lemmas.pow2_exp_1 max_limb max_limb;
-  (* FproductLemmas.helper_lemma_10 max_limb;   *)
-  Curve.Parameters.parameters_lemma_1 (); 
-  (* FproductLemmas.helper_lemma_11 platform_wide (log_2 norm_length) max_limb;  *)
-  Math.Lemmas.pow2_increases_1 platform_wide max_wide
+let lemma_swap p1 a p2 b : Lemma ((p1 * a) * (p2 * b) = p1 * p2 * (a * b)) = ()
 
-val max_limb_lemma2: h:heap -> a:bigint{live h a} -> b:bigint{live h b} -> i:nat{i < length a} -> ctr:nat{ctr < length b} -> Lemma
-    (requires (S64.v (get h a i) < pow2 max_limb /\ S64.v (get h b ctr) < pow2 max_limb))
-    (ensures (S64.v (get h a i) * S64.v (get h b ctr) < pow2 platform_wide))
-let max_limb_lemma2 h a b i ctr =
-  max_limb_lemma (S64.v (get h a i)) (S64.v (get h b ctr))
 
-(* #reset-options *)
+private let lemma_multiplication061
+  (a0:int) (a1:int) (a2:int) (a3:int) (a4:int)
+  (b0:int) (b1:int) (b2:int) (b3:int) (b4:int) :
+  Lemma (
+    (pow2 51*a1)*b0+(pow2 51*a1)*(pow2 51*b1)+(pow2 51*a1)*(pow2 102*b2)+(pow2 51*a1)*(pow2 153*b3)+(pow2 51*a1)*(pow2 204*b4)
+    = pow2 51 * (a1 * b0) + pow2 102 * (a1 * b1) + pow2 153 * (a1 * b2) + pow2 204 * (a1 * b3) + pow2 255 * (a1 * b4) )
+  = pow2_plus 51 51;
+    pow2_plus 51 102;
+    pow2_plus 51 153;
+    pow2_plus 51 204;
+    lemma_swap (pow2 51) a1 (pow2 51) b1;
+    lemma_swap (pow2 51) a1 (pow2 102) b2;
+    lemma_swap (pow2 51) a1 (pow2 153) b3;
+    lemma_swap (pow2 51) a1 (pow2 204) b4
 
-val is_scalar_product_lemma:
-  h0:heap -> h1:heap -> a:bigint{live h0 a /\ length a >= norm_length} -> s:s64 -> res:bigint_wide{live h1 res /\ length res >= norm_length} ->
-  Lemma
-    (requires (Curve.Fscalar.isScalarProduct h0 h1 0 norm_length a s res))
-    (ensures (isScalarProduct h1 res h0 a s))
-let is_scalar_product_lemma h0 h1 a s res = ()
 
-val multiplication_step_0: a:bigint -> b:bigint -> ctr:u32{w ctr<norm_length/\w ctr<2*norm_length-1} -> 
-  c:bigint_wide{disjoint a c /\ disjoint b c} -> 
-  tmp:bigint_wide{disjoint a tmp /\ disjoint b tmp /\ disjoint c tmp} -> STL unit 
-     (requires (fun h -> norm h a /\ norm h b /\ live h c /\ live h tmp
-        /\ length c >= 2*norm_length -1
-	/\ maxValueNorm h a < pow2 max_limb
-	/\ maxValueNorm h b < pow2 max_limb
-	/\ maxValue_wide h c (length c) <= w ctr * maxValueNorm h a * maxValueNorm h b
-       ))
-     (ensures (fun h0 _ h1 ->
-       norm h0 a /\ norm h0 b /\ live h0 c /\ live h1 tmp
-       /\ live h0 tmp /\ length tmp = length tmp
-       /\ length c >= 2*norm_length-1 /\ length tmp >= norm_length
-       /\ modifies_1 tmp h0 h1
-       /\ isScalarProduct h1 tmp h0 a (get h0 b (w ctr))
-       /\ eval_wide h1 tmp norm_length = eval h0 a norm_length * vv (get h0 b (w ctr)) ))
-let multiplication_step_0 a b ctr c tmp = 
-  admit(); // OK
-  let h0 = ST.get() in
-  let s = index b ctr in 
-  assert(forall (n:nat). {:pattern (vv (get h0 b n))} n < norm_length ==> vv (get h0 b n) <= pow2 max_limb); 
-  assert(forall (n:nat). n = w ctr ==> n < norm_length); 
-  assert(True /\ vv s < pow2 max_limb); 
-  assert(forall (i:nat). {:pattern (vv  (get h0 a i))} 
-	   i < norm_length ==> vv (get h0 a i) < pow2 max_limb);
-  assert(vv s < pow2 max_limb); 
-  cut(forall (i:nat). (i < norm_length) ==> vv (get h0 a i) * vv s < pow2 platform_wide); 
-  Curve.Fscalar.scalar_multiplication_tr tmp a s 0ul; 
-  let h1 = ST.get() in
-  cut(True /\ vv s = vv (get h0 b (w ctr))); 
-  assert(Fscalar.isScalarProduct h0 h1 0 norm_length a s tmp); 
-  is_scalar_product_lemma h0 h1 a s tmp;
-  Curve.Fscalar.theorem_scalar_multiplication h0 h1 a s norm_length tmp
+#reset-options "--z3timeout 20 --initial_fuel 0 --max_fuel 0"
 
-#reset-options
+private let lemma_multiplication062
+  (a0:int) (a1:int) (a2:int) (a3:int) (a4:int)
+  (b0:int) (b1:int) (b2:int) (b3:int) (b4:int) :
+  Lemma (
+    (pow2 102*a2)*b0+(pow2 102*a2)*(pow2 51*b1)+(pow2 102*a2)*(pow2 102*b2)+(pow2 102*a2)*(pow2 153*b3)+(pow2 102*a2)*(pow2 204*b4)
+    = pow2 102  * (a2 * b0) + pow2 153  * (a2 * b1) + pow2 204 * (a2 * b2) + pow2 255 * (a2 * b3) + pow2 306 * (a2 * b4) )
+  = pow2_plus 102 51;
+    pow2_plus 102 102;
+    pow2_plus 102 153;
+    pow2_plus 102 204;
+    lemma_swap (pow2 102) a2 (pow2 51) b1;
+    lemma_swap (pow2 102) a2 (pow2 102) b2;
+    lemma_swap (pow2 102) a2 (pow2 153) b3;
+    lemma_swap (pow2 102) a2 (pow2 204) b4
 
-val std_lemma: h0:heap -> h1:heap -> a:bigint -> tmp:bigint_wide{disjoint a tmp} ->Lemma
-    (requires (norm h0 a /\ live h1 tmp /\ modifies_1 tmp h0 h1))
-    (ensures (norm h1 a))
-let std_lemma h0 h1 a tmp = 
-  admit(); // OK
-  (* no_upd_lemma h0 h1 a (only tmp);  *)
-  cut(forall (i:nat). {:pattern (vv (get h1 a i))} i < norm_length ==> vv (get h1 a i) = vv (get h0 a i)); 
-  cut(True /\ live h1 a); cut(True /\ length a >= norm_length); cut (True /\ templ = templ); 
-  cut(forall (i:nat). {:pattern (norm h1 a)} i < norm_length ==> vv (get h1 a i) < pow2 (templ i)); 
-  cut(norm h1 a)
- 
-assume val max_wide_lemma:
-  x:nat{x <= norm_length} -> Lemma (x * pow2 max_wide < pow2 platform_wide)
+#reset-options "--z3timeout 20 --initial_fuel 0 --max_fuel 0"
 
-#reset-options
+private let lemma_multiplication063
+  (a0:int) (a1:int) (a2:int) (a3:int) (a4:int)
+  (b0:int) (b1:int) (b2:int) (b3:int) (b4:int) :
+  Lemma (
+    (pow2 153*a3)*b0+(pow2 153*a3)*(pow2 51*b1)+(pow2 153*a3)*(pow2 102*b2)+(pow2 153*a3)*(pow2 153*b3)+(pow2 153*a3)*(pow2 204*b4)
+    = pow2 153  * (a3 * b0) + pow2 204 * (a3 * b1) + pow2 255 * (a3 * b2) + pow2 306 * (a3 * b3) + pow2 357 * (a3 * b4) )
+  = pow2_plus 153 51;
+    pow2_plus 153 102;
+    pow2_plus 153 153;
+    pow2_plus 153 204;
+    lemma_swap (pow2 153) a3 (pow2 51) b1;
+    lemma_swap (pow2 153) a3 (pow2 102) b2;
+    lemma_swap (pow2 153) a3 (pow2 153) b3;
+    lemma_swap (pow2 153) a3 (pow2 204) b4
 
-val lemma_helper_00: unit -> Lemma (forall (a:nat) (b:nat) (c:nat) (d:nat). (a <= b /\ c <= d) ==> a * c <= b * d)
-let lemma_helper_00 () = 
-  admit(); // OK
-  ()
+#reset-options "--z3timeout 20 --initial_fuel 0 --max_fuel 0"
 
-val lemma_helper_01: a:int -> b:int -> c:int -> Lemma (a * (b+c) + b + c = (a+1) * (b+c))
-let lemma_helper_01 a b c = 
-  admit(); // OK
-  ()
+private let lemma_multiplication064
+  (a0:int) (a1:int) (a2:int) (a3:int) (a4:int)
+  (b0:int) (b1:int) (b2:int) (b3:int) (b4:int) :
+  Lemma (
+    (pow2 204*a4)*b0+(pow2 204*a4)*(pow2 51*b1)+(pow2 204*a4)*(pow2 102*b2) +(pow2 204*a4)*(pow2 153*b3)+(pow2 204*a4)*(pow2 204*b4)
+    = pow2 204 * (a4 * b0) + pow2 255 * (a4 * b1) + pow2 306 * (a4 * b2) + pow2 357 * (a4 * b3) + pow2 408 * (a4 * b4) )
+  = pow2_plus 204 51;
+    pow2_plus 204 102;
+    pow2_plus 204 153;
+    pow2_plus 204 204;
+    lemma_swap (pow2 204) a4 (pow2 51) b1;
+    lemma_swap (pow2 204) a4 (pow2 102) b2;
+    lemma_swap (pow2 204) a4 (pow2 153) b3;
+    lemma_swap (pow2 204) a4 (pow2 204) b4
 
-val lemma_helper_02: a:nat -> b:nat -> c:nat -> Lemma (requires (b <= c)) (ensures (a*b <= a*c))
-let lemma_helper_02 a b c = 
-  admit(); // OK
-  ()
+#reset-options "--z3timeout 20 --initial_fuel 0 --max_fuel 0"
 
-val multiplication_step_lemma_0010:  h0:heap -> h1:heap -> a:bigint -> b:bigint -> 
-  ctr:nat{ctr<norm_length} -> c:bigint_wide{disjoint a c /\ disjoint b c} -> 
-  tmp:bigint_wide{disjoint a tmp /\ disjoint b tmp /\ disjoint c tmp} -> Lemma
-     (requires (
-       norm h0 a /\ norm h0 b /\ live h0 c /\ live h1 tmp
-       /\ length c >= 2*norm_length -1
-       /\ maxValueNorm h0 a < pow2 max_limb /\ maxValueNorm h0 b < pow2 max_limb
-       /\ maxValue_wide h0 c (length c) <= ctr * maxValueNorm h0 a * maxValueNorm h0 b
-       /\ modifies_1 tmp h0 h1
-       /\ isScalarProduct h1 tmp h0 a (get h0 b ctr) ))
-     (ensures (live h1 tmp /\ norm h0 a /\ norm h0 b
-       /\ length tmp >= norm_length
-       /\ (forall (i:nat). {:pattern (v (get h1 tmp i))} i < norm_length ==> v (get h1 tmp i) <= maxValueNorm h0 a * maxValueNorm h0 b) ))
-let multiplication_step_lemma_0010 h0 h1 a b ctr c tmp = 
-  admit(); // OK
-  lemma_helper_00 ()
+private let lemma_multiplication06
+  (a0:int) (a1:int) (a2:int) (a3:int) (a4:int)
+  (b0:int) (b1:int) (b2:int) (b3:int) (b4:int) :
+  Lemma (
+    a0*b0+a0*(pow2 51*b1)+a0*(pow2 102*b2)+a0*(pow2 153*b3)+a0*(pow2 204*b4)
+      +(pow2 51*a1)*b0+(pow2 51*a1)*(pow2 51*b1)+(pow2 51*a1)*(pow2 102*b2)+(pow2 51*a1)*(pow2 153*b3)+(pow2 51*a1)*(pow2 204*b4)
+      +(pow2 102*a2)*b0+(pow2 102*a2)*(pow2 51*b1)+(pow2 102*a2)*(pow2 102*b2)+(pow2 102*a2)*(pow2 153*b3)+(pow2 102*a2)*(pow2 204*b4)
+      +(pow2 153*a3)*b0+(pow2 153*a3)*(pow2 51*b1)+(pow2 153*a3)*(pow2 102*b2)+(pow2 153*a3)*(pow2 153*b3)+(pow2 153*a3)*(pow2 204*b4)
+      +(pow2 204*a4)*b0+(pow2 204*a4)*(pow2 51*b1)+(pow2 204*a4)*(pow2 102*b2) +(pow2 204*a4)*(pow2 153*b3)+(pow2 204*a4)*(pow2 204*b4)
+    =              (a0 * b0) + pow2 51  * (a0 * b1) + pow2 102  * (a0 * b2) + pow2 153  * (a0 * b3) + pow2 204 * (a0 * b4)
+      + pow2 51  * (a1 * b0) + pow2 102  * (a1 * b1) + pow2 153  * (a1 * b2) + pow2 204 * (a1 * b3) + pow2 255 * (a1 * b4)
+      + pow2 102  * (a2 * b0) + pow2 153  * (a2 * b1) + pow2 204 * (a2 * b2) + pow2 255 * (a2 * b3) + pow2 306 * (a2 * b4)
+      + pow2 153  * (a3 * b0) + pow2 204 * (a3 * b1) + pow2 255 * (a3 * b2) + pow2 306 * (a3 * b3) + pow2 357 * (a3 * b4)
+      + pow2 204 * (a4 * b0) + pow2 255 * (a4 * b1) + pow2 306 * (a4 * b2) + pow2 357 * (a4 * b3) + pow2 408 * (a4 * b4) )
+  = lemma_multiplication060 a0 a1 a2 a3 a4 b0 b1 b2 b3 b4;
+    lemma_multiplication061 a0 a1 a2 a3 a4 b0 b1 b2 b3 b4;
+    lemma_multiplication062 a0 a1 a2 a3 a4 b0 b1 b2 b3 b4;
+    lemma_multiplication063 a0 a1 a2 a3 a4 b0 b1 b2 b3 b4;
+    lemma_multiplication064 a0 a1 a2 a3 a4 b0 b1 b2 b3 b4
 
-val multiplication_step_lemma_001: h0:heap -> h1:heap -> a:bigint -> b:bigint -> 
-  ctr:nat{ctr<norm_length} -> c:bigint_wide{disjoint a c /\ disjoint b c} -> 
-  tmp:bigint_wide{disjoint a tmp /\ disjoint b tmp /\ disjoint c tmp} -> 
-  Lemma
-     (requires (
-       norm h0 a /\ norm h0 b /\ live h0 c /\ live h1 tmp
-       /\ (length c >= 2*norm_length -1)
-       /\ (maxValueNorm h0 a < pow2 max_limb) /\ (maxValueNorm h0 b < pow2 max_limb)
-       /\ (maxValue_wide h0 c (length c)  <= ctr * maxValueNorm h0 a * maxValueNorm h0 b)
-       /\ modifies_1 tmp h0 h1
-       /\ isScalarProduct h1 tmp h0 a (get h0 b ctr) ))
-     (ensures (live h1 c /\ live h1 tmp /\ ctr+norm_length <= length c
-       /\ Curve.FsumWide.willNotOverflow h1 ctr 0 norm_length 0 c tmp ))
-let multiplication_step_lemma_001 h0 h1 a b ctr c tmp =
-  admit(); // OK
-  multiplication_step_lemma_0010 h0 h1 a b ctr c tmp;
-  Math.Axioms.distributivity_add_left ctr 1 (maxValueNorm h0 a * maxValueNorm h0 b);
-  cut(forall (i:nat). {:pattern (v (get h1 c i))} i < norm_length ==> v (get h1 c (i+ctr)) <= ctr * maxValueNorm h0 a * maxValueNorm h0 b);
-  cut (True /\ ctr * maxValueNorm h0 a * maxValueNorm h0 b + maxValueNorm h0 a * maxValueNorm h0 b
-    = (ctr+1) * (maxValueNorm h0 a * maxValueNorm h0 b) );
-  cut (forall (i:nat). {:pattern (v (get h1 c (i+ctr)) + v (get h1 tmp i))} i < norm_length ==> v (get h1 c (i+ctr)) + v (get h1 tmp i) <= (ctr+1) * (maxValueNorm h0 a * maxValueNorm h0 b));
-  auxiliary_lemma_3 h0 h0 h1 a b ctr c;
-  assert ((maxValueNorm h0 a * maxValueNorm h0 b) <= pow2 max_wide);
-  lemma_helper_02 (ctr+1) (maxValueNorm h0 a * maxValueNorm h0 b) (pow2 max_wide);
-  cut(True /\ (ctr+1) * (maxValueNorm h0 a * maxValueNorm h0 b) <= (ctr + 1) * pow2 max_wide);
-  max_wide_lemma (ctr+1); 
-  assert((ctr+1) * pow2 max_wide < pow2 platform_wide);
-  (* FproductLemmas.helper_lemma_4 (maxValueNorm h0 a) (maxValueNorm h0 b); *)
-  (* FproductLemmas.helper_lemma_4 (ctr+1) (maxValueNorm h0 a * maxValueNorm h0 b); *)
-  (* FproductLemmas.helper_lemma_4 (ctr+1) (pow2 max_wide); *)
-  (* FproductLemmas.ineq_lemma_2 ((ctr+1) * (maxValueNorm h0 a * maxValueNorm h0 b)) ((ctr+1) * pow2 max_wide) (pow2 platform_wide); *)
-  assert ((ctr+1) * (maxValueNorm h0 a * maxValueNorm h0 b) < pow2 platform_wide);
-  assert(forall (i:nat). i < norm_length ==> v (get h1 c (i+ctr)) + v (get h1 tmp i) <= (ctr+1) * (maxValueNorm h0 a * maxValueNorm h0 b) ==> v (get h1 c (i+ctr)) + v (get h1 tmp i) < pow2 platform_wide); 
-  cut(forall (i:nat). i < norm_length ==> v (get h1 c (i+ctr)) + v (get h1 tmp i) < pow2 platform_wide); 
-  assert(FsumWide.willNotOverflow h1 ctr 0 norm_length 0 c tmp)
+#reset-options "--z3timeout 20 --initial_fuel 0 --max_fuel 0"
 
-val multiplication_step_lemma_01: h0:heap -> h1:heap -> a:bigint -> b:bigint ->
-  ctr:nat{ctr<norm_length} -> c:bigint_wide{disjoint a c /\ disjoint b c} ->
-  tmp:bigint_wide{disjoint a tmp /\ disjoint b tmp /\ disjoint c tmp} ->
-  Lemma
-     (requires (norm h0 a /\ norm h0 b /\ live h0 c /\ live h1 tmp
-        /\ (length c >= 2*norm_length -1)
-	/\ (maxValueNorm h0 a < pow2 max_limb) /\ (maxValueNorm h0 b < pow2 max_limb)
-	/\ (maxValue_wide h0 c (length c) <= ctr * maxValueNorm h0 a * maxValueNorm h0 b)
-	/\ modifies_1 tmp h0 h1
-	/\ isScalarProduct h1 tmp h0 a (get h0 b ctr) ))
-     (ensures (
-       (live h1 c) /\ (live h1 tmp) /\ (ctr+norm_length <= length c) 
-       /\ (norm h1 a) /\ (norm h1 b)
-       /\ (0+norm_length <= length tmp)
-       /\ FsumWide.willNotOverflow h1 ctr 0 norm_length 0 c tmp
-     ))
-let multiplication_step_lemma_01 h0 h1 a b ctr c tmp =
-  admit(); // OK
-  (* no_upd_lemma h0 h1 c (only tmp);  *)
-  cut(True /\ length c >= ctr + norm_length); 
-  std_lemma h0 h1 a tmp;
-  std_lemma h0 h1 b tmp; 
-  multiplication_step_lemma_001 h0 h1 a b ctr c tmp
+private let lemma_multiplication07
+  (a0:int) (a1:int) (a2:int) (a3:int) (a4:int)
+  (b0:int) (b1:int) (b2:int) (b3:int) (b4:int) :
+  Lemma ((a0 + pow2 51 * a1 + pow2 102 * a2 + pow2 153 * a3 + pow2 204 * a4)
+    * (b0 + pow2 51 * b1 + pow2 102 * b2 + pow2 153 * b3 + pow2 204 * b4)
+    =              (a0 * b0) + pow2 51  * (a0 * b1) + pow2 102  * (a0 * b2) + pow2 153  * (a0 * b3) + pow2 204 * (a0 * b4)
+      + pow2 51  * (a1 * b0) + pow2 102  * (a1 * b1) + pow2 153  * (a1 * b2) + pow2 204 * (a1 * b3) + pow2 255 * (a1 * b4)
+      + pow2 102  * (a2 * b0) + pow2 153  * (a2 * b1) + pow2 204 * (a2 * b2) + pow2 255 * (a2 * b3) + pow2 306 * (a2 * b4)
+      + pow2 153  * (a3 * b0) + pow2 204 * (a3 * b1) + pow2 255 * (a3 * b2) + pow2 306 * (a3 * b3) + pow2 357 * (a3 * b4)
+      + pow2 204 * (a4 * b0) + pow2 255 * (a4 * b1) + pow2 306 * (a4 * b2) + pow2 357 * (a4 * b3) + pow2 408 * (a4 * b4) )
+  = lemma_multiplication05 a0 a1 a2 a3 a4 b0 b1 b2 b3 b4;
+    lemma_multiplication06 a0 a1 a2 a3 a4 b0 b1 b2 b3 b4
 
-val partial_equality_lemma: h0:heap -> h1:heap -> c:bigint_wide{live h0 c /\ live h1 c /\ length c = length c} -> ctr:nat{ ctr + norm_length <= length c} ->
-  Lemma
-    (requires (FsumWide.isNotModified h0 h1 ctr norm_length 0 c))
-    (ensures (partialEquality h1 c h0 c ctr))
-let partial_equality_lemma h0 h1 c ctr = 
-  admit(); // OK
-  ()
+#reset-options "--z3timeout 20 --initial_fuel 0 --max_fuel 0"
 
-val lemma_helper_10: a:nat -> b:nat -> c:nat -> Lemma (a <= a + (b * c))
-let lemma_helper_10 a b c = 
-  admit(); // OK
-  ()
+private let lemma_multiplication08
+  (a0:int) (a1:int) (a2:int) (a3:int) (a4:int)
+  (b0:int) (b1:int) (b2:int) (b3:int) (b4:int) :
+  Lemma (
+    a0 * b0 + pow2 51  * (a1 * b0 + a0 * b1)
+	    + pow2 102  * (a2 * b0 + a1 * b1 + a0 * b2)
+	    + pow2 153  * (a3 * b0 + a2 * b1 + a1 * b2 + a0 * b3)
+	    + pow2 204 * (a4 * b0 + a3 * b1 + a2 * b2 + a1 * b3 + a0 * b4)
+	    + pow2 255 * (a4 * b1 + a3 * b2 + a2 * b3 + a1 * b4)
+	    + pow2 306 * (a4 * b2 + a3 * b3 + a2 * b4)
+	    + pow2 357 * (a4 * b3 + a3 * b4)
+	    + pow2 408 * (a4 * b4)
+    =              (a0 * b0) + pow2 51  * (a0 * b1) + pow2 102  * (a0 * b2) + pow2 153  * (a0 * b3) + pow2 204 * (a0 * b4)
+      + pow2 51  * (a1 * b0) + pow2 102  * (a1 * b1) + pow2 153  * (a1 * b2) + pow2 204 * (a1 * b3) + pow2 255 * (a1 * b4)
+      + pow2 102  * (a2 * b0) + pow2 153  * (a2 * b1) + pow2 204 * (a2 * b2) + pow2 255 * (a2 * b3) + pow2 306 * (a2 * b4)
+      + pow2 153  * (a3 * b0) + pow2 204 * (a3 * b1) + pow2 255 * (a3 * b2) + pow2 306 * (a3 * b3) + pow2 357 * (a3 * b4)
+      + pow2 204 * (a4 * b0) + pow2 255 * (a4 * b1) + pow2 306 * (a4 * b2) + pow2 357 * (a4 * b3) + pow2 408 * (a4 * b4) )
+  = lemma_multiplication00 (pow2 51) (a1 * b0) (a0 * b1);
+    lemma_multiplication01 (pow2 102) (a2 * b0) (a1 * b1) (a0 * b2);
+    lemma_multiplication02 (pow2 153) (a3 * b0) (a2 * b1) (a1 * b2) (a0 * b3);
+    lemma_multiplication03 (pow2 204) (a4 * b0) (a3 * b1) (a2 * b2) (a1 * b3) (a0 * b4);
+    lemma_multiplication02 (pow2 255) (a4 * b1) (a3 * b2) (a2 * b3) (a1 * b4);
+    lemma_multiplication01 (pow2 306) (a4 * b2) (a3 * b3) (a2 * b4);
+    lemma_multiplication00 (pow2 357) (a4 * b3) (a3 * b4)
 
-#reset-options
 
-val max_value_lemma_1: h0:heap -> h1:heap -> h2:heap -> a:bigint -> b:bigint -> 
-  ctr:nat{ctr < norm_length} -> c:bigint_wide{disjoint a c /\ disjoint b c} -> 
-  tmp:bigint_wide{disjoint a tmp /\ disjoint b tmp /\ disjoint c tmp} -> Lemma
-    (requires (
-      norm h0 a /\ norm h0 b /\ live h0 c /\ live h1 tmp /\ live h2 c /\ live h1 c
-      /\ length c >= 2 * norm_length - 1
-      /\ modifies_1 tmp h0 h1
-      /\ maxValue_wide h0 c (length c) <= ctr * maxValueNorm h0 a * maxValueNorm h0 b
-      /\ (forall (i:nat). {:pattern (v (get h2 c (i+ctr)))} 
-	  i < norm_length ==> v (get h2 c (i+ctr)) = v (get h0 c (i+ctr)) + (vv (get h0 a i) * vv (get h0 b ctr)))
-      /\ (forall (i:nat). {:pattern (v (get h2 c i))} ((i < ctr \/ i >= norm_length + ctr) /\ i < length c) ==> v (get h2 c i) = v (get h0 c i))
-    ))
-    (ensures ( norm h0 a /\ norm h0 b /\ live h2 c
-       /\ (maxValue_wide h2 c (length c) <= (ctr+1) * maxValueNorm h0 a * maxValueNorm h0 b)))
-let max_value_lemma_1 h0 h1 h2 a b ctr c tmp =
-  admit(); // OK
-  cut(forall (i:nat). {:pattern (vv (get h0 a i))} 
-    i < norm_length ==> vv (get h0 a i) <= maxValueNorm h0 a);
-  cut(forall (i:nat). {:pattern (vv (get h0 b i))} 
-	   i < norm_length ==> vv (get h0 b i) <= maxValueNorm h0 b);
-  cut(forall (i:nat). {:pattern (v (get h0 c i))} i < length c ==> v (get h0 c i) <= maxValue_wide h0 c (length c));
-  cut(forall (i:nat). {:pattern (v (get h0 c (i+ctr)))} 
-	   i < norm_length ==> v (get h0 c (i+ctr)) <= maxValue_wide h0 c (length c));
-  (* FproductLemmas.ineq_lemma (); *)
-  assert(forall (a:nat) (b':nat) (c:nat) (d:nat). {:pattern (vv (get h0 b ctr))} a <= c /\ b' <= d ==> a * b' <= c * d);
-  assert(vv (get h0 b ctr) <= maxValueNorm h0 b);
-  cut(forall (i:nat). {:pattern (vv (get h0 a i) * vv (get h0 b ctr))} i < norm_length ==>
-    (vv (get h0 a i)) <= maxValueNorm h0 a /\ vv (get h0 b ctr) <= maxValueNorm h0 b); 
-  cut(forall (i:nat). {:pattern (vv (get h0 a i) * vv (get h0 b ctr))} i < norm_length ==>
-    (vv (get h0 a i) * vv (get h0 b ctr)) <= maxValueNorm h0 a * maxValueNorm h0 b);
-  assert(forall (a':nat) (b':nat) (c':nat) (d:nat). {:pattern (maxValue_wide h0 c (length c) + (maxValueNorm h0 a * maxValueNorm h0 b))} a' <= c' /\ b' <= d ==> a' + b' <= c' + d); 
-  cut(forall (i:nat). {:pattern (v (get h0 c (i+ctr)) + (vv (get h0 a i) * vv (get h0 b ctr)))} i < norm_length ==> v (get h0 c (i+ctr)) + (vv (get h0 a i) * vv (get h0 b ctr)) <= maxValue_wide h0 c (length c) + (maxValueNorm h0 a * maxValueNorm h0 b)); 
-  assert(forall (i:nat). i < norm_length ==> v (get h2 c (i+ctr)) <= maxValue_wide h0 c (length c) + (maxValueNorm h0 a * maxValueNorm h0 b)); 
-  assert(forall (i:nat). {:pattern (i < length c)} i < length c ==>
-	   ((i >= ctr /\ i < norm_length+ctr) \/ ((i < ctr \/ i >= norm_length + ctr) /\ i < length c))); 
-  cut(forall (i:nat). (i>=ctr /\ i<norm_length+ctr) ==> (i-ctr>=0 /\ i-ctr < norm_length /\ ((i-ctr)+ctr) = i)); 
-  cut(forall (i:nat). {:pattern (i >= ctr /\ i < norm_length+ctr)} (i >= ctr /\ i < norm_length+ctr) ==> v (get h2 c i) <= maxValue_wide h0 c (length c) + (maxValueNorm h0 a * maxValueNorm h0 b));
-  assert(forall (i:nat). {:pattern ((i < ctr \/ i >= norm_length + ctr) /\ i < length c)} 
-    ((i < ctr \/ i >= norm_length + ctr) /\ i < length c) ==> v (get h2 c i) <= maxValue_wide h0 c (length c)); 
-    lemma_helper_10 (maxValue_wide h0 c (length c)) (maxValueNorm h0 a) (maxValueNorm h0 b); 
-  cut(True /\ maxValue_wide h0 c (length c) <= maxValue_wide h0 c (length c) + (maxValueNorm h0 a * maxValueNorm h0 b)); 
-  assert(forall (i:nat).  ((i < ctr \/ i >= norm_length + ctr) /\ i < length c) ==> v (get h2 c i) <= maxValue_wide h0 c (length c)); 
-  assert(forall (i:nat). {:pattern (v (get h2 c i))} ((i < ctr \/ i >= norm_length + ctr) /\ i < length c) ==> v (get h2 c i) <= maxValue_wide h0 c (length c) + (maxValueNorm h0 a * maxValueNorm h0 b)); 
-  cut(forall (i:nat). {:pattern(maxValue_wide h0 c (length c) + (maxValueNorm h0 a * maxValueNorm h0 b))}
-    i < length c ==> 
-      ((i >= ctr /\ i < norm_length+ctr) \/ ((i < ctr \/ i >= norm_length + ctr) /\ i < length c)) ==>
-	v (get h2 c i) <= maxValue_wide h0 c (length c) + (maxValueNorm h0 a * maxValueNorm h0 b)); 
-  Math.Axioms.paren_mul_right ctr (maxValueNorm h0 a) (maxValueNorm h0 b); 
-  cut(True /\ maxValue_wide h0 c (length c) <= ctr * (maxValueNorm h0 a * maxValueNorm h0 b)); 
-  (* FproductLemmas.factorise_lemma (maxValueNorm h0 a * maxValueNorm h0 b) ctr; *)
-  assert(True /\ maxValue_wide h0 c (length c) + (maxValueNorm h0 a * maxValueNorm h0 b) <= (ctr+1) * (maxValueNorm h0 a * maxValueNorm h0 b)); 
-  assert(forall (i:nat). 
-    i < length c ==> 
-	v (get h2 c i) <= (ctr+1) * (maxValueNorm h0 a * maxValueNorm h0 b)); 
-  assert(maxValue_wide h2 c (length c) <= (ctr+1) * (maxValueNorm h0 a * maxValueNorm h0 b))
+#reset-options "--z3timeout 20 --initial_fuel 0 --max_fuel 0"
 
-val max_value_lemma: h0:heap -> h1:heap -> h2:heap -> a:bigint -> b:bigint -> 
-  ctr:nat{ctr < norm_length} -> c:bigint_wide{disjoint a c /\ disjoint b c} -> 
-  tmp:bigint_wide{disjoint a tmp /\ disjoint b tmp /\ disjoint c tmp} ->
-  Lemma
-    (requires (
-      norm h0 a /\ norm h0 b /\ live h0 c /\ live h1 tmp /\ live h2 c /\ live h1 c
-      /\ modifies_1 tmp h0 h1
-      /\ length c >= 2 * norm_length - 1
-      /\ (maxValue_wide h0 c (length c) <= ctr * maxValueNorm h0 a * maxValueNorm h0 b)
-      /\ isScalarProduct h1 tmp h0 a (get h0 b ctr)
-      /\ FsumWide.isSum h1 h2 ctr 0 norm_length 0 c tmp
-      /\ FsumWide.isNotModified h1 h2 ctr norm_length 0 c))
-    (ensures (norm h0 a /\ norm h0 b /\ live h2 c
-       /\ maxValue_wide h2 c (length c) <= (ctr+1) * maxValueNorm h0 a * maxValueNorm h0 b))
-let max_value_lemma h0 h1 h2 a b ctr c tmp =
-  admit(); // OK
-  cut(forall (i:nat). {:pattern (v (get h1 tmp i))} i < norm_length ==> v (get h1 tmp i) = vv (get h0 a i) * vv (get h0 b ctr)); 
-  cut(forall (i:nat). {:pattern (v (get h2 c (i+ctr)))} i < norm_length ==> v (get h2 c (i+ctr)) = v (get h1 c (i+ctr)) + v (get h1 tmp i)); 
-  cut(forall (i:nat). {:pattern (v (get h2 c i))} 
-    ((i < ctr \/ i >= norm_length + ctr) /\ i < length c) ==> v (get h2 c i) = v (get h1 c i)); 
-  (* no_upd_lemma h0 h1 c (only tmp); *)
-  cut(forall (i:nat). {:pattern (v (get h1 c i))} i < length c ==> v (get h1 c i) = v (get h0 c i)); 
-  cut(forall (i:nat). {:pattern (v (get h1 tmp i))}
-    i < norm_length ==> v (get h1 tmp i) = vv (get h0 a i) * vv (get h0 b ctr)); 
-  cut(forall (i:nat). i < norm_length ==> v (get h2 c (i+ctr)) = v (get h0 c (i+ctr)) + (vv (get h0 a i) * vv (get h0 b ctr))); 
-  max_value_lemma_1 h0 h1 h2 a b ctr c tmp
+private let lemma_multiplication0
+  (a0:int) (a1:int) (a2:int) (a3:int) (a4:int)
+  (b0:int) (b1:int) (b2:int) (b3:int) (b4:int) :
+  Lemma (
+    (a0 + pow2 51 * a1 + pow2 102 * a2 + pow2 153 * a3 + pow2 204 * a4)
+    * (b0 + pow2 51 * b1 + pow2 102 * b2 + pow2 153 * b3 + pow2 204 * b4) =
+    a0 * b0 + pow2 51  * (a1 * b0 + a0 * b1)
+	    + pow2 102  * (a2 * b0 + a1 * b1 + a0 * b2)
+	    + pow2 153  * (a3 * b0 + a2 * b1 + a1 * b2 + a0 * b3)
+	    + pow2 204 * (a4 * b0 + a3 * b1 + a2 * b2 + a1 * b3 + a0 * b4)
+	    + pow2 255 * (a4 * b1 + a3 * b2 + a2 * b3 + a1 * b4)
+	    + pow2 306 * (a4 * b2 + a3 * b3 + a2 * b4)
+	    + pow2 357 * (a4 * b3 + a3 * b4)
+	    + pow2 408 * (a4 * b4) )
+  = lemma_multiplication07 a0 a1 a2 a3 a4 b0 b1 b2 b3 b4;
+    lemma_multiplication08 a0 a1 a2 a3 a4 b0 b1 b2 b3 b4
 
-let modifies_2 c tmp h0 h1 =
-  HyperHeap.modifies_just (Set.union (Set.singleton (frameOf c)) (Set.singleton (frameOf tmp))) h0.h h1.h
-  (* /\ modifies_buf (frameOf c) (only c ++ tmp) h0 h1 *)
-  (* /\ modifies_buf (frameOf tmp) (only c ++ tmp) h0 h1 *)
-  /\ h0.tip = h1.tip
 
-val standardized_lemma: h0:heap -> h1:heap -> h2:heap -> a:bigint -> c:bigint_wide{disjoint a c} -> 
-  tmp:bigint_wide{disjoint a tmp /\ disjoint c tmp} -> Lemma
-    (requires (norm h0 a /\ live h0 c /\ live h1 tmp /\ live h1 c
-	/\ modifies_1 tmp h0 h1
-	/\ modifies_1 c h1 h2 ))
-     (ensures (norm h0 a /\ norm h2 a /\ live h0 c  /\ live h1 tmp /\ live h2 tmp
-       /\ modifies_2 c tmp h0 h2 ))
-let standardized_lemma h0 h1 h2 a c tmp =
-  admit(); // OK
-  (* cut(modifies !{getRef c,getRef tmp} h0 h2);  *)
-  (* no_upd_lemma h0 h2 a (only c ++ tmp); *)
-  (* no_upd_lemma h1 h2 tmp (only c); *)
-  cut(forall (i:nat). {:pattern (vv (get h2 a i))} i < norm_length ==> vv (get h2 a i) = vv (get h0 a i));
-  cut(True /\ live h2 a); cut(True /\ length a >= norm_length); cut (True /\ templ = templ); 
-  cut(forall (i:nat). {:pattern (norm h2 a)} i < norm_length ==> vv (get h2 a i) < pow2 (templ i)); 
-  cut(norm h2 a)
+#reset-options "--z3timeout 20 --initial_fuel 0 --max_fuel 0"
 
-val length_lemma: h0:heap -> h1:heap -> h2:heap -> c:bigint_wide -> ctr:nat{ctr < norm_length} ->
-  tmp:bigint_wide{disjoint c tmp} -> Lemma 
-     (requires (live h0 c /\ live h1 tmp /\ live h1 c /\ live h0 tmp
-	/\ length c >= 2 * norm_length - 1
-	/\ modifies_1 tmp h0 h1
-	/\ live h2 c /\ live h2 tmp
-	/\ ctr+norm_length <= length c
-	/\ modifies_1 c h1 h2 ))
-     (ensures (live h0 c /\ live h2 c  /\ live h0 tmp /\ live h2 tmp
-       /\ length c >= 2 * norm_length - 1
-       /\ modifies_2 c tmp h0 h2 ))
-let length_lemma h0 h1 h2 c ctr tmp =
-  admit(); // OK
-  (* no_upd_lemma h0 h1 c (only tmp); *)
-  (* no_upd_lemma h1 h2 tmp (only c) *)
-  ()
+val lemma_multiplication1:
+  h0:mem -> h1:mem ->
+  c:bigint_wide{length c >= 2*norm_length-1} ->
+  a:bigint -> b:bigint ->
+  Lemma (requires (isMultiplication h0 h1 a b c))
+	(ensures  (isMultiplication h0 h1 a b c
+	  /\ eval_wide h1 c (2*norm_length-1) = eval h0 a norm_length * eval h0 b norm_length))
+let lemma_multiplication1 h0 h1 c a b =
+  let a0 = v (get h0 a 0) in
+  let a1 = v (get h0 a 1) in
+  let a2 = v (get h0 a 2) in
+  let a3 = v (get h0 a 3) in
+  let a4 = v (get h0 a 4) in
+  let b0 = v (get h0 b 0) in
+  let b1 = v (get h0 b 1) in
+  let b2 = v (get h0 b 2) in
+  let b3 = v (get h0 b 3) in
+  let b4 = v (get h0 b 4) in
+  lemma_eval_bigint_wide_9 h1 c;
+  lemma_eval_bigint_5 h0 a;
+  lemma_eval_bigint_5 h0 b;
+  lemma_multiplication0 a0 a1 a2 a3 a4 b0 b1 b2 b3 b4
 
-val lemma_helper_20:   h0:heap -> h1:heap -> h2:heap -> a:bigint -> b:bigint -> ctr:nat{ctr < norm_length} -> c:bigint_wide{disjoint a c /\ disjoint b c} -> tmp:bigint_wide{disjoint a tmp /\ disjoint b tmp /\ disjoint c tmp} -> Lemma 
-  (requires(live h2 tmp /\ live h1 tmp /\ live h1 c /\ live h2 c /\ length c >= 2 * norm_length - 1
-    /\ FsumWide.isSum h1 h2 ctr 0 norm_length 0 c tmp 
-    ))
-  (ensures (live h2 tmp /\ live h1 tmp /\ live h2 c /\ live h1 c /\ length c >= 2 * norm_length - 1
-    /\ FsumWide.isSum h1 h2 ctr 0 norm_length 0 c tmp
-    /\ storesSum h2 c h1 c h1 tmp ctr norm_length ))
-let lemma_helper_20 h0 h1 h2 a b ctr c tmp = ()
 
-val multiplication_step_lemma_02: h0:heap -> h1:heap -> h2:heap -> a:bigint -> b:bigint -> 
-  ctr:u32{w ctr < norm_length} ->
-  c:bigint_wide{disjoint a c /\ disjoint b c} ->
-  tmp:bigint_wide{disjoint a tmp /\ disjoint b tmp /\ disjoint c tmp} -> Lemma 
-     (requires (norm h0 a /\ norm h0 b /\ live h0 c /\ live h1 tmp /\ live h1 c	/\ live h0 tmp
-	/\ length c >= 2 * norm_length - 1
-	/\ maxValueNorm h0 a < pow2 max_limb
-	/\ maxValueNorm h0 b < pow2 max_limb
-	/\ maxValue_wide h0 c (length c) <= w ctr * maxValueNorm h0 a * maxValueNorm h0 b
-	// After fscalar
-	/\ modifies_1 tmp h0 h1
-	/\ isScalarProduct h1 tmp h0 a (get h0 b (w ctr))
-        /\ eval_wide h1 tmp norm_length = eval h0 a norm_length * vv (get h0 b (w ctr))
- 	// After fsum
-	/\ live h2 c /\ live h2 tmp
-	/\ w ctr+norm_length <= length c
-	/\ modifies_1 c h1 h2
-	/\ FsumWide.isSum h1 h2 (w ctr) 0 norm_length 0 c tmp
-	/\ FsumWide.isNotModified h1 h2 (w ctr) norm_length 0 c ))
-     (ensures (norm h0 a /\ norm h2 a /\ norm h0 b /\ norm h2 b
-       /\ live h0 c /\ live h2 c  /\ live h0 tmp /\ live h2 tmp  /\ length c >= 2 * norm_length - 1
-       /\ modifies_2 c tmp h0 h2
-       /\ maxValueNorm h0 a < pow2 max_limb
-       /\ maxValueNorm h0 b < pow2 max_limb
-       /\ maxValue_wide h0 c (length c) <= w ctr * maxValueNorm h0 a * maxValueNorm h0 b
-       /\ maxValue_wide h2 c (length c) <= (w ctr+1) * maxValueNorm h0 a * maxValueNorm h0 b
-       /\ eval_wide h2 c (2*norm_length-1) = eval_wide h0 c (2*norm_length-1) + pow2 (bitweight (templ) (w ctr)) * eval h0 a norm_length * vv (get h0 b (w ctr)) ))
-let multiplication_step_lemma_02 h0 h1 h2 a b ctr c tmp =
-  admit(); // OK timeout 50
-  assert(forall (i:nat). (i >= norm_length + w ctr /\ i < 2 * norm_length - 1) ==>
-  	   v (get h2 c i) = v (get h1 c i));
-  (* eval_partial_eq_lemma h1 h2 c c (norm_length+ctr) (2*norm_length-1);  *)
-  (* no_upd_lemma h0 h1 c (only tmp); *)
-  (* cut(forall (i:nat). i < length c ==> v (get h0 c i) = v (get h1 c i));  *)
-  (* eval_eq_lemma h0 h1 c c (2*norm_length-1); *)
-  (* eval_eq_lemma h0 h1 c c (norm_length+ctr); *)
-  cut(True /\ eval_wide h2 c (2*norm_length-1) - eval_wide h2 c (norm_length+w ctr) = eval_wide h0 c (2*norm_length-1) - eval_wide h0 c (norm_length+w ctr)); 
-  (* cut (True /\ eval h1 tmp norm_length = eval h0 a norm_length * v (get h0 b ctr));  *)
-  lemma_helper_20 h0 h1 h2 a b (w ctr) c tmp;
-  (* cut (storesSum h2 c h1 c h1 tmp ctr norm_length); admit() *)
-  partial_equality_lemma h1 h2 c (w ctr); 
-  cut (partialEquality h2 c h1 c (w ctr)); 
-  multiplication_step_lemma h1 h2 c tmp c (w ctr) norm_length; 
-  cut (True /\ eval_wide h2 c (norm_length+w ctr) = eval_wide h1 c (norm_length+w ctr) + pow2 (bitweight (templ) (w ctr)) * eval h0 a norm_length * vv (get h0 b (w ctr)));
-  cut (True /\ eval_wide h2 c (norm_length+w ctr) = eval_wide h0 c (norm_length+w ctr) + pow2 (bitweight (templ) (w ctr)) * eval h0 a norm_length * vv (get h0 b (w ctr)));
-  cut (True /\ eval_wide h2 c (2*norm_length-1) = eval_wide h0 c (2*norm_length-1) + pow2 (bitweight (templ) (w ctr)) * eval h0 a norm_length * vv (get h0 b (w ctr)));
-  max_value_lemma h0 h1 h2 a b (w ctr) c tmp; 
-  Math.Axioms.paren_mul_right (w ctr+1) (maxValueNorm h0 a) (maxValueNorm h0 b);
-  (* assert(maxValue_wid h2 c <= (ctr+1) * maxValueNorm h0 a * maxValueNorm h0 b);  *)
-  standardized_lemma h0 h1 h2 a c tmp; 
-  standardized_lemma h0 h1 h2 b c tmp;
-  length_lemma h0 h1 h2 c (w ctr) tmp;
-  ()
-  
-#reset-options
+#reset-options "--z3timeout 100 --initial_fuel 0 --max_fuel 0"
 
-val multiplication_step_p1: a:bigint -> b:bigint -> ctr:u32{w ctr<norm_length} -> 
-  c:bigint_wide{disjoint a c /\ disjoint b c} -> 
-  tmp:bigint_wide{disjoint a tmp /\ disjoint b tmp /\ disjoint c tmp} -> STL unit 
-     (requires (fun h -> norm h a /\ norm h b /\ live h c /\ live h tmp
-        /\ length c >= 2*norm_length -1
-	/\ maxValueNorm h a < pow2 max_limb
-	/\ maxValueNorm h b < pow2 max_limb
-	/\ maxValue_wide h c (length c) <= w ctr * maxValueNorm h a * maxValueNorm h b
-	/\ eval_wide h c (2*norm_length-1) = eval h a (norm_length) * eval h b (w ctr) ))
-     (ensures (fun h0 u h1 -> norm h0 a /\ norm h0 b /\ live h0 c /\ live h0 tmp
-       /\ norm h1 a /\ norm h1 b /\ live h1 c /\ live h1 tmp
-       /\ length c >= 2*norm_length -1
-       /\ modifies_2 c tmp h0 h1
-       /\ maxValue_wide h0 c (length c) <= w ctr * maxValueNorm h0 a * maxValueNorm h0 b
-       /\ maxValue_wide h1 c (length c) <= (w ctr+1) * (maxValueNorm h0 a * maxValueNorm h0 b)
-       /\ eval_wide h0 c (2*norm_length-1) = eval h0 a (norm_length) * eval h0 b (w ctr)
-       /\ (eval_wide h1 c (2*norm_length-1) = eval_wide h0 c (2*norm_length-1) + pow2 (bitweight (templ) (w ctr)) * eval h0 a norm_length * vv (get h0 b (w ctr)))
-     ))
-let multiplication_step_p1 a b ctr c tmp =
-  admit(); // OK
-  let h0 = ST.get() in
-  multiplication_step_0 a b ctr c tmp; 
-  let h1 = ST.get() in
-  multiplication_step_lemma_01 h0 h1 a b (w ctr) c tmp; 
-  FsumWide.fsum_index c ctr tmp 0ul nlength 0ul; 
-  let h2 = ST.get() in 
-  multiplication_step_lemma_02 h0 h1 h2 a b ctr c tmp
+let lemma_mul_ineq (a:nat) (b:nat) c d : Lemma (requires (a < c /\ b < d))
+					    (ensures  (a * b < c * d))
+  = ()
 
-val helper_lemma_6: h0:heap -> h1:heap -> a:bigint -> b:bigint -> ctr:nat{ctr < norm_length} -> 
-  c:bigint_wide{disjoint a c /\ disjoint b c} -> 
-  tmp:bigint_wide{disjoint a tmp /\ disjoint b tmp /\ disjoint c tmp} -> Lemma
-     (requires (norm h0 a /\ norm h0 b /\ live h0 c /\ length c >= 2 * norm_length - 1))
-    (ensures (norm h0 a /\ norm h0 b /\ live h0 c /\ length c >= 2 * norm_length - 1
-       /\ eval_wide h0 c (2*norm_length-1) + pow2 (bitweight (templ) ctr) * eval h0 a (norm_length) * vv (get h0 b ctr)  = eval h0 a (norm_length) * vv (get h0 b ctr) * pow2 (bitweight (templ) ctr) + eval_wide h0 c (2*norm_length-1) ))
-let helper_lemma_6 h0 h1 a b ctr c tmp = ()
-  (* FproductLemmas.helper_lemma_5 (eval h0 c (2*norm_length-1)) (pow2 (bitweight (templ) ctr)) (eval h0 a norm_length) (v (get h0 b ctr)) *)
+val lemma_multiplication2:
+  h0:mem -> h1:mem ->
+  c:bigint_wide{length c >= 2*norm_length-1} ->
+  a:bigint -> b:bigint ->
+  Lemma (requires (norm h0 a /\ norm h0 b /\ isMultiplication h0 h1 a b c))
+	(ensures  (norm h0 a /\ norm h0 b /\ isMultiplication h0 h1 a b c
+	  /\ maxValue_wide h1 c 9 <= norm_length * pow2 102))
+let lemma_multiplication2 h0 h1 c a b =
+  pow2_plus 51 51;
+  let a0 = v (get h0 a 0) in
+  let a1 = v (get h0 a 1) in
+  let a2 = v (get h0 a 2) in
+  let a3 = v (get h0 a 3) in
+  let a4 = v (get h0 a 4) in
+  let b0 = v (get h0 b 0) in
+  let b1 = v (get h0 b 1) in
+  let b2 = v (get h0 b 2) in
+  let b3 = v (get h0 b 3) in
+  let b4 = v (get h0 b 4) in
+  lemma_mul_ineq a0 b0 (pow2 51) (pow2 51);
+  lemma_mul_ineq a0 b1 (pow2 51) (pow2 51);
+  lemma_mul_ineq a0 b2 (pow2 51) (pow2 51);
+  lemma_mul_ineq a0 b3 (pow2 51) (pow2 51);
+  lemma_mul_ineq a0 b4 (pow2 51) (pow2 51);
+  lemma_mul_ineq a1 b0 (pow2 51) (pow2 51);
+  lemma_mul_ineq a1 b1 (pow2 51) (pow2 51);
+  lemma_mul_ineq a1 b2 (pow2 51) (pow2 51);
+  lemma_mul_ineq a1 b3 (pow2 51) (pow2 51);
+  lemma_mul_ineq a1 b4 (pow2 51) (pow2 51);
+  lemma_mul_ineq a2 b0 (pow2 51) (pow2 51);
+  lemma_mul_ineq a2 b1 (pow2 51) (pow2 51);
+  lemma_mul_ineq a2 b2 (pow2 51) (pow2 51);
+  lemma_mul_ineq a2 b3 (pow2 51) (pow2 51);
+  lemma_mul_ineq a2 b4 (pow2 51) (pow2 51);
+  lemma_mul_ineq a3 b0 (pow2 51) (pow2 51);
+  lemma_mul_ineq a3 b1 (pow2 51) (pow2 51);
+  lemma_mul_ineq a3 b2 (pow2 51) (pow2 51);
+  lemma_mul_ineq a3 b3 (pow2 51) (pow2 51);
+  lemma_mul_ineq a3 b4 (pow2 51) (pow2 51);
+  lemma_mul_ineq a4 b0 (pow2 51) (pow2 51);
+  lemma_mul_ineq a4 b1 (pow2 51) (pow2 51);
+  lemma_mul_ineq a4 b2 (pow2 51) (pow2 51);
+  lemma_mul_ineq a4 b3 (pow2 51) (pow2 51);
+  lemma_mul_ineq a4 b4 (pow2 51) (pow2 51);
+  let open Hacl.UInt128 in
+  assert(v (get h1 c 0) < pow2 102);
+  assert(v (get h1 c 1) < 2*pow2 102);
+  assert(v (get h1 c 2) < 3*pow2 102);
+  assert(v (get h1 c 3) < 4*pow2 102);
+  assert(v (get h1 c 4) < 5*pow2 102);
+  assert(v (get h1 c 5) < 4*pow2 102);
+  assert(v (get h1 c 6) < 3*pow2 102);
+  assert(v (get h1 c 7) < 2*pow2 102);
+  assert(v (get h1 c 8) < pow2 102);
+  maxValue_wide_bound_lemma_aux h1 c (2*norm_length-1) (5*pow2 102)
 
-(* Code : does 1 step of the multiplication (1 scalar multiplication), 
-   and infers the appropriate properties on sizes, values and evaluated
-   values for the resulting bigint *)
-val multiplication_step: a:bigint -> b:bigint -> ctr:u32{w ctr < norm_length} -> 
-  c:bigint_wide{disjoint a c /\ disjoint b c} -> 
-  tmp:bigint_wide{disjoint a tmp /\ disjoint b tmp /\ disjoint c tmp} -> STL unit  
-     (requires (fun h -> norm h a /\ norm h b /\ live h c /\ live h tmp
-	/\ length c >= 2 * norm_length - 1
-	/\ maxValueNorm h a < pow2 max_limb
-	/\ maxValueNorm h b < pow2 max_limb
-	/\ maxValue_wide h c (length c) <= w ctr * maxValueNorm h a * maxValueNorm h b
-	/\ eval_wide h c (2*norm_length-1) = eval h a (norm_length) * eval h b (w ctr) ))
-     (ensures (fun h0 u h1 -> norm h0 a /\ norm h1 a /\ norm h0 b /\ norm h1 b
-       /\ live h0 c /\ live h1 c  /\ live h0 tmp /\ live h1 tmp
-       /\ length c >= 2 * norm_length - 1
-       /\ modifies_2 c tmp h0 h1
-       /\ maxValueNorm h0 a < pow2 max_limb
-       /\ maxValueNorm h0 b < pow2 max_limb
-       /\ maxValue_wide h0 c (length c) <= w ctr * maxValueNorm h0 a * maxValueNorm h0 b
-       /\ maxValue_wide h1 c (length c) <= (w ctr+1) * maxValueNorm h0 a * maxValueNorm h0 b
-       /\ eval_wide h0 c (2*norm_length-1) = eval h0 a (norm_length) * eval h0 b (w ctr)
-       /\ eval_wide h1 c (2*norm_length-1) = eval h0 a (norm_length) * vv (get h0 b (w ctr)) * pow2 (bitweight (templ) (w ctr)) + eval_wide h0 c (2*norm_length-1)
-     ))
-let multiplication_step a b ctr c tmp =
-  let h0 = ST.get() in
-  multiplication_step_p1 a b ctr c tmp;  
-  let h1 = ST.get() in
-  helper_lemma_6 h0 h1 a b (w ctr) c tmp
-  
-(* Lemma : factorizes "eval" equation *)
-val multiplication_step_lemma_03: h0:heap -> h1:heap -> a:bigint{norm h0 a} -> b:bigint{norm h0 b} ->
-  ctr:pos{ctr <= norm_length} -> c:bigint_wide{live h1 c /\ length c >= 2*norm_length-1} -> Lemma
-    (requires (eval_wide h1 c (2*norm_length-1) = (eval h0 a (norm_length) * vv (get h0 b (norm_length - ctr))) * pow2 (bitweight (templ) (norm_length - ctr)) + eval h0 a (norm_length) * eval h0 b (norm_length - ctr) ))
-    (ensures (eval_wide h1 c (2*norm_length-1) = eval h0 a (norm_length) * eval h0 b (norm_length - ctr + 1)))
-let multiplication_step_lemma_03 h0 h1 a b ctr c =
-  admit(); // OK
-  let t = templ in 
-  Math.Axioms.paren_mul_left (eval h0 a norm_length) (vv (get h0 b (norm_length - ctr))) (pow2 (bitweight t (norm_length - ctr))); 
-  cut (True /\ eval_wide h1 c (2*norm_length-1) = eval h0 a norm_length * vv (get h0 b (norm_length - ctr)) * pow2 (bitweight t (norm_length - ctr)) + eval h0 a norm_length * eval h0 b (norm_length - ctr) ); 
-  Math.Axioms.swap_mul (vv (get h0 b (norm_length - ctr))) (pow2 (bitweight t (norm_length - ctr))); 
-  cut (True /\ eval_wide h1 c (2*norm_length-1) = eval h0 a norm_length * pow2 (bitweight t (norm_length - ctr)) * vv (get h0 b (norm_length - ctr)) + eval h0 a norm_length * eval h0 b (norm_length - ctr) ) ; 
-  Math.Axioms.distributivity_add_right (eval h0 a norm_length) (pow2 (bitweight t (norm_length - ctr)) * vv (get h0 b (norm_length - ctr))) (eval h0 b (norm_length - ctr)); 
-  cut (True /\ eval_wide h1 c (2*norm_length-1) = eval h0 a norm_length * (pow2 (bitweight t (norm_length - ctr)) * vv (get h0 b (norm_length - ctr)) + eval h0 b (norm_length - ctr))); 
-  eval_def h0 b (norm_length-ctr+1)
 
-val helper_lemma_7: ctr:pos{ctr < norm_length} -> Lemma 
-    (requires (True))
-    (ensures (norm_length - ctr + 1 >= 0 /\ norm_length - ctr + 1 <= norm_length))
-    [SMTPat (norm_length - ctr + 1)]
-let helper_lemma_7 ctr = ()
-  (* FproductLemmas.helper_lemma_7 norm_length ctr *)
+#reset-options "--z3timeout 5 --initial_fuel 0 --max_fuel 0"
 
-val multiplication_aux_lemma: h0:heap -> h1:heap -> a:bigint -> b:bigint -> 
-  ctr:pos{ctr <= norm_length} -> c:bigint_wide{disjoint a c /\ disjoint b c} -> 
-  tmp:bigint_wide{disjoint a tmp /\ disjoint b tmp /\ disjoint c tmp} -> Lemma
-    (requires (norm h0 a /\ norm h1 a /\ norm h0 b /\ norm h1 b
-       /\ live h0 c /\ live h1 c  /\ live h0 tmp /\ live h1 tmp 
-       /\ length c >= 2 * norm_length - 1
-       /\ ((norm_length - ctr) < norm_length) 
-       /\ modifies_2 c tmp h0 h1
-       /\ maxValueNorm h0 a < pow2 max_limb
-       /\ maxValueNorm h0 b < pow2 max_limb
-       /\ maxValue_wide h0 c (length c) <= (norm_length - ctr) * maxValueNorm h0 a * maxValueNorm h0 b
-       /\ maxValue_wide h1 c (length c) <= ((norm_length - ctr)+1) * maxValueNorm h0 a * maxValueNorm h0 b
-       /\ eval_wide h0 c (2*norm_length-1) = eval h0 a (norm_length) * eval h0 b (norm_length - ctr)
-       /\ eval_wide h1 c (2*norm_length-1) = eval h0 a (norm_length) * vv (get h0 b (norm_length - ctr)) * pow2 (bitweight (templ) (norm_length - ctr)) + eval_wide h0 c (2*norm_length-1) ))
-    (ensures (norm h1 a /\ norm h1 b /\ live h1 c /\ live h1 tmp /\ (length c >= 2 * norm_length - 1)
-	/\ maxValueNorm h1 a < pow2 max_limb
-	/\ maxValueNorm h1 b < pow2 max_limb
-	/\ maxValue_wide h1 c (length c) <= (norm_length - ctr + 1) * (maxValueNorm h1 a * maxValueNorm h1 b)
-	/\ eval_wide h1 c (2*norm_length-1) = eval h1 a (norm_length) * eval h1 b (norm_length - ctr + 1) ))
-let multiplication_aux_lemma h0 h1 a b ctr c tmp =
-  admit(); // OK timeout 50
-  (* no_upd_lemma h0 h1 a (only c ++ tmp); *)
-  maxValueNorm_eq_lemma h0 h1 a a; 
-  eval_eq_lemma h0 h1 a a norm_length;
-  (* no_upd_lemma h0 h1 b (only c ++ tmp);  *)
-  maxValueNorm_eq_lemma h0 h1 b b; 
-  eval_eq_lemma h0 h1 b b (norm_length - ctr);
-  eval_eq_lemma h0 h1 b b (norm_length - ctr + 1);
-  cut((maxValueNorm h1 a = maxValueNorm h0 a)
-       /\ (maxValueNorm h1 b = maxValueNorm h0 b)); 
-  cut((norm_length - ctr)+1 = norm_length - ctr + 1 /\ True);
-  cut(eval h0 a norm_length = eval h1 a norm_length /\ eval h0 b (norm_length-ctr) = eval h1 b (norm_length - ctr) /\ eval h0 b (norm_length - ctr + 1) = eval h1 b (norm_length - ctr + 1) /\ vv (get h0 b (norm_length - ctr)) = vv (get h1 b (norm_length - ctr)));
-  Math.Axioms.paren_mul_right (norm_length - ctr + 1) (maxValueNorm h1 a) (maxValueNorm h1 b);
-  cut(norm_length - ctr + 1 > 0 /\ length b >= norm_length - ctr + 1);
-  eval_def h0 b (norm_length - ctr + 1); 
-  assert (eval_wide h0 c (2*norm_length-1) = eval h0 a (norm_length) * eval h0 b (norm_length - ctr));
-  assert (eval_wide h1 c (2*norm_length-1) = eval h0 a (norm_length) * vv (get h0 b (norm_length - ctr)) * pow2 (bitweight (templ) (norm_length - ctr)) + eval_wide h0 c (2*norm_length-1));
-  assert (eval_wide h1 c (2*norm_length-1) = eval h0 a (norm_length) * vv (get h0 b (norm_length - ctr)) * pow2 (bitweight (templ) (norm_length - ctr)) + (eval h0 a (norm_length) * eval h0 b (norm_length - ctr))); 
-  (* FproductLemmas.helper_lemma_12 (eval h0 a norm_length) (v (get h0 b (norm_length - ctr))) (pow2 (bitweight (templ) (norm_length - ctr))) (eval h0 b (norm_length - ctr)) *)
-  ()
-  
-val multiplication_aux_lemma_2: h0:heap -> h1:heap -> h2:heap -> a:bigint -> b:bigint -> 
-  ctr:nat{ctr <= norm_length} -> c:bigint_wide{disjoint a c /\ disjoint b c} -> 
-  tmp:bigint_wide{disjoint a tmp /\ disjoint b tmp /\ disjoint c tmp} -> Lemma 
-    (requires ((norm h0 a) /\ (norm h0 b) /\ (live h1 c) /\ (live h1 tmp)
-       /\ (norm h1 a) /\ (norm h1 b) /\ (live h1 c) /\ (live h1 tmp)
-       /\ (norm h2 a) /\ (norm h2 b) /\ (live h2 c) /\ (live h2 tmp)
-       /\ (length c >= 2 * norm_length - 1)
-       /\ modifies_2 c tmp h0 h1
-       /\ modifies_2 c tmp h1 h2
-       /\ eval_wide h2 c (2*norm_length-1) = eval h1 a (norm_length) * eval h1 b (norm_length) ))
-    (ensures (norm h0 a /\ norm h0 b /\ live h1 c /\ norm h2 a /\ norm h2 b /\ live h2 c
-       /\ length c >= 2 * norm_length - 1
-       /\ modifies_2 c tmp h0 h2
-       /\ eval_wide h2 c (2*norm_length-1) = eval h0 a (norm_length) * eval h0 b (norm_length) ))
-let multiplication_aux_lemma_2 h0 h1 h2 a b ctr c tmp =
-  admit(); // OK
-    cut(modifies_2 c tmp h0 h2);
-    (* no_upd_lemma h0 h1 a (only c ++ tmp);  *)
-    (* no_upd_lemma h0 h1 b (only c ++ tmp);  *)
-    eval_eq_lemma h0 h1 a a norm_length; 
-    eval_eq_lemma h0 h1 b b norm_length
-
-(* Code : tail recursive calls to run the multiplication *)
-val multiplication_aux: a:bigint -> b:bigint -> ctr:u32{w ctr <= norm_length} -> 
-  c:bigint_wide{disjoint a c /\ disjoint b c} ->
-  tmp:bigint_wide{disjoint a tmp /\ disjoint b tmp /\ disjoint c tmp} -> STL unit
-     (requires (fun h -> (norm h a) /\ (norm h b) /\ (live h c) /\ (live h tmp)
-	/\ (length c >= 2 * norm_length - 1)
-	/\ (maxValueNorm h a < pow2 max_limb)
-	/\ (maxValueNorm h b < pow2 max_limb)
-	/\ (maxValue_wide h c (length c) <= (norm_length - w ctr) * (maxValueNorm h a * maxValueNorm h b))
-	/\ (eval_wide h c (2*norm_length-1) = eval h a (norm_length) * eval h b (norm_length - w ctr))))
-     (ensures (fun h0 u h1 -> 
-       (norm h0 a) /\ (norm h0 b) /\ (live h0 c) /\ (live h0 tmp)
-       /\ (norm h1 a) /\ (norm h1 b) /\ (live h1 c) /\ (live h1 tmp)
-       /\ (length c >= 2 * norm_length - 1)
-       /\ (modifies_2 c tmp h0 h1)
-       /\ (maxValueNorm h0 a < pow2 max_limb)
-       /\ (maxValueNorm h0 b < pow2 max_limb)
-       /\ (eval_wide h1 c (2*norm_length-1) = eval h0 a (norm_length) * eval h0 b (norm_length))
-       /\ (maxValue_wide h1 c (length c) <= norm_length * (maxValueNorm h0 a * maxValueNorm h0 b))
-     ))
-let rec multiplication_aux a b ctr c tmp = 
-  let h0 = ST.get() in
-  if U32.eq ctr 0ul then ()
-  else begin
-    (* FproductLemmas.helper_lemma_8 norm_length ctr; *)
-    multiplication_step a b (nlength -| ctr) c tmp;
-    let h1 = ST.get() in    
-    multiplication_aux_lemma h0 h1 a b (w ctr) c tmp;
-    multiplication_aux a b (ctr-|1ul) c tmp;
-    let h2 = ST.get() in
-    multiplication_aux_lemma_2 h0 h1 h2 a b (w ctr) c tmp
-  end
-
-#reset-options
-
-(* val helper_lemma_16: h0:heap -> h1:heap -> a:bigint -> mods:FStar.Set.set aref -> *)
-(*   Lemma (requires (norm h0 a /\ modifies mods h0 h1 /\ not(FStar.Set.mem (Ref (getRef a)) mods))) *)
-(* 	(ensures (norm h1 a)) *)
-(* let helper_lemma_16 h0 h1 a mods =  *)
-(*   no_upd_lemma h0 h1 a mods *)
-
-val helper_lemma_13: h0:heap -> h1:heap -> a:bigint ->
-  Lemma 
-    (requires ((norm h0 a) /\ modifies Set.empty h0 h1))
-    (ensures (norm h0 a /\ norm h1 a
-	      /\ live h1 a /\ length a >= norm_length
-	      /\ maxValueNorm h0 a = maxValueNorm h1 a
-	      /\ eval h0 a norm_length = eval h1 a norm_length))
-let helper_lemma_13 h0 h1 a = 
-  admit(); // OK
-  (* no_upd_lemma h0 h1 a (!{}); *)
-  (* helper_lemma_16 h0 h1 a !{}; *)
-  eval_eq_lemma h0 h1 a a norm_length; 
-  maxValueNorm_eq_lemma h0 h1 a a
-
-val helper_lemma_15: h0:heap -> h1:heap -> c:bigint_wide ->
-  Lemma
-    (requires (live h0 c /\ null_wide h0 c /\ length c >= 2 * norm_length - 1 /\ modifies Set.empty h0 h1))
-    (ensures (live h1 c /\ null_wide h1 c /\ maxValue_wide h1 c (length c) <= 0 /\ length c >= 2 * norm_length - 1 /\ eval_wide h1 c (2*norm_length-1) = 0))
-let helper_lemma_15 h0 h1 c =
-  admit(); // OK
-  (* no_upd_lemma h0 h1 c !{}; () *)
-  (* eval_null h1 c (2*norm_length - 1);  *)
-  (* max_value_of_null_lemma h1 c *)
-  ()
-
-#reset-options
-
-val multiplication_lemma_1: h0:heap -> h1:heap -> c:bigint_wide -> a:bigint{disjoint c a} -> 
-  b:bigint{disjoint c b} -> Lemma
-     (requires (norm h0 a /\ norm h0 b /\ live h0 c /\ null_wide h0 c /\ length c >= 2*norm_length-1
-	/\ maxValueNorm h0 a < pow2 max_limb
-	/\ maxValueNorm h0 b < pow2 max_limb
-	/\ HyperStack.modifies Set.empty h0 h1
-	/\ h0.tip = h1.tip))
-     (ensures (norm h1 a /\ norm h1 b /\ live h1 c /\ null_wide h1 c /\ length c >= 2*norm_length-1
-	/\ maxValueNorm h1 a < pow2 max_limb
-	/\ maxValueNorm h1 b < pow2 max_limb
-	/\ maxValue_wide h1 c (length c) <= (norm_length - norm_length) * (maxValueNorm h1 a * maxValueNorm h1 b)
-	/\ (eval_wide h1 c (2*norm_length-1) = eval h1 a (norm_length) * eval h1 b (norm_length - norm_length)) ))
-let multiplication_lemma_1 h0 h1 c a b =
-  helper_lemma_13 h0 h1 a;
-  helper_lemma_13 h0 h1 b;
-  helper_lemma_15 h0 h1 c;   
-  cut(norm_length - norm_length = 0 /\ True); 
-  (* FproductLemmas.auxiliary_lemma_90 (norm_length);  *)
-  (* FproductLemmas.helper_lemma_13 (maxValueNorm h1 a * maxValueNorm h1 b);  *)
-  cut(True /\ eval h1 b 0 = 0); 
-  (* FproductLemmas.helper_lemma_13 (eval h1 a norm_length) *)
-  ()
-
-val helper_lemma_14: h0:heap -> h1:heap -> h2:heap -> c:bigint_wide -> tmp:bigint_wide{disjoint c tmp} ->
-  Lemma
-    (requires (live h0 c /\ live h2 c /\ ~(contains h0 (tmp))
-	       /\ modifies Set.empty h0 h1 /\ live h1 tmp /\ modifies_2 c tmp h1 h2))
-    (ensures (modifies_1 c h0 h2))
-let helper_lemma_14 h0 h1 h2 c tmp =
-  admit(); // OK
-  ()
-
-val multiplication_lemma_2: h0:heap -> h1:heap -> h2:heap -> c:bigint_wide ->  a:bigint{disjoint c a} -> 
-  b:bigint{disjoint c b} -> tmp:bigint_wide{disjoint a tmp /\ disjoint b tmp /\ disjoint c tmp} -> Lemma
-     (requires (norm h0 a /\ norm h0 b /\ live h0 c /\ null_wide h0 c /\ length c >= 2*norm_length-1
-	/\ maxValueNorm h0 a < pow2 max_limb
-	/\ maxValueNorm h0 b < pow2 max_limb
-	/\ HyperStack.modifies Set.empty h0 h1 /\ h0.tip = h1.tip 
-	/\ ~(contains h0 (tmp)) /\ contains h1 (tmp)
-	/\ norm h1 a /\ norm h1 b /\ live h1 c /\ null_wide h1 c
-	/\ length c >= 2*norm_length-1
-	/\ maxValueNorm h1 a < pow2 max_limb
-	/\ maxValueNorm h1 b < pow2 max_limb
-	/\ maxValue_wide h1 c (length c) <= (norm_length - norm_length) * (maxValueNorm h1 a * maxValueNorm h1 b)
-	/\ eval_wide h1 c (2*norm_length-1) = eval h1 a (norm_length) * eval h1 b (norm_length - norm_length)
-       /\ norm h2 a /\ norm h2 b /\ live h2 c
-       /\ length c >= 2*norm_length-1
-       /\ modifies_2 c tmp h1 h2
-       /\ eval_wide h2 c (2*norm_length-1) = eval h1 a (norm_length) * eval h1 b (norm_length)
-       /\ maxValue_wide h2 c (length c) <= norm_length * (maxValueNorm h1 a * maxValueNorm h1 b)
-     ))
-     (ensures (
-       (norm h0 a) /\ (norm h0 b) /\ (live h0 c)
-       /\ (norm h2 a) /\ (norm h2 b) /\ (live h2 c)
-       /\ (length c >= 2*norm_length-1) /\ (length c >= 2*norm_length-1)
-       /\ (null_wide h0 c) /\ (modifies_1 c h0 h2)
-       /\ (maxValueNorm h0 a < pow2 max_limb)
-       /\ (maxValueNorm h0 b < pow2 max_limb)
-       /\ (eval_wide h2 c (2*norm_length-1) = eval h0 a (norm_length) * eval h0 b (norm_length))
-       /\ (maxValue_wide h2 c (length c) <= norm_length * maxValueNorm h0 a * maxValueNorm h0 b) ))
-let multiplication_lemma_2 h0 h1 h2 c a b tmp =
-  admit(); // OK
-  helper_lemma_14 h0 h1 h2 c tmp;
-  helper_lemma_13 h0 h1 a;
-  helper_lemma_13 h0 h1 b
-
-(* Code : core multiplication function *)
-val multiplication: c:bigint_wide -> a:bigint{disjoint c a} -> b:bigint{disjoint c b} -> STL unit
-     (requires (fun h -> norm h a /\ norm h b /\ live h c /\ null_wide h c /\ length c >= 2*norm_length-1
-	/\ maxValueNorm h a < pow2 max_limb
-	/\ maxValueNorm h b < pow2 max_limb ))
-     (ensures (fun h0 u h1 -> norm h0 a /\ norm h0 b /\ live h0 c /\ norm h1 a /\ norm h1 b /\ live h1 c
-       /\ length c >= 2*norm_length-1
-       /\ null_wide h0 c /\ modifies_1 c h0 h1
-       /\ maxValueNorm h0 a < pow2 max_limb
-       /\ maxValueNorm h0 b < pow2 max_limb
-       /\ eval_wide h1 c (2*norm_length-1) = eval h0 a (norm_length) * eval h0 b (norm_length)
-       /\ maxValue_wide h1 c (length c) <= norm_length * maxValueNorm h0 a * maxValueNorm h0 b ))
-let multiplication c a b =
-  admit(); // OK
-  let h0 = ST.get() in
-  let tmp = create (Hacl.UInt128.of_string "0") nlength in
-  let h1 = ST.get() in
-  (* assert(modifies Set.empty h0 h1);  *)
-  multiplication_lemma_1 h0 h1 c a b; 
-  cut(True /\ length tmp >= norm_length);
-  (* constant_template_lemma c a;  *)
-  multiplication_aux a b nlength c tmp; 
-  let h2 = ST.get() in 
-  multiplication_lemma_2 h0 h1 h2 c a b tmp
+val lemma_multiplication:
+  h0:mem ->
+  h1:mem ->
+  c:bigint_wide{length c >= 2*norm_length-1} ->
+  a:bigint{disjoint c a} ->
+  b:bigint{disjoint c b} ->
+  Lemma (requires (norm h0 a /\ norm h0 b /\ live h1 c /\ isMultiplication h0 h1 a b c))
+	(ensures  (norm h0 a /\ norm h0 b /\ live h1 c /\ isMultiplication h0 h1 a b c
+	  /\ eval_wide h1 c (2*norm_length-1) = eval h0 a norm_length * eval h0 b norm_length
+	  /\ maxValue_wide h1 c (2*norm_length-1) <= norm_length * pow2 102))
+let lemma_multiplication h0 h1 c a b =
+  lemma_multiplication1 h0 h1 c a b;
+  lemma_multiplication2 h0 h1 c a b
