crypto/ec/Hacl.EC.Curve25519.Bignum.Fproduct.fst
@@ -15,6 +15,8 @@ open Hacl.EC.Curve25519.Parameters
 open Hacl.EC.Curve25519.Bigint
 open Hacl.EC.Curve25519.Utils
 
+open Hacl.EC.Curve25519.Bignum.Fproduct.Lemmas
+
 #reset-options "--initial_fuel 0 --max_fuel 0"
 
 (* Module abbreviations *)
@@ -30,51 +32,51 @@ module H128  = Hacl.UInt128
 
 let u51 = x:H64.t{v x < pow2 51}
 
-let op_Star_Bar (x:H64.t) (y:H64.t) : H128.t = H128.mul_wide x y
+(* let op_Star_Bar (x:H64.t) (y:H64.t) : H128.t = H128.mul_wide x y *)
 
-let isMultiplication (h0:mem) (h1:mem) (a:bigint) (b:bigint) (c:bigint_wide) : GTot Type0 =
-  live h0 a /\ live h0 b /\ live h1 c
-  /\ length a >= norm_length /\ length b >= norm_length /\ length c >= 2*norm_length-1
-  /\ (
-    let a0 = v (get h0 a 0) in let a1 = v (get h0 a 1) in let a2 = v (get h0 a 2) in
-    let a3 = v (get h0 a 3) in let a4 = v (get h0 a 4) in let b0 = v (get h0 b 0) in
-    let b1 = v (get h0 b 1) in let b2 = v (get h0 b 2) in let b3 = v (get h0 b 3) in
-    let b4 = v (get h0 b 4) in
-    let open Hacl.UInt128 in
-    let c0 = v (get h1 c 0) in let c1 = v (get h1 c 1) in
-    let c2 = v (get h1 c 2) in let c3 = v (get h1 c 3) in let c4 = v (get h1 c 4) in
-    let c5 = v (get h1 c 5) in let c6 = v (get h1 c 6) in let c7 = v (get h1 c 7) in
-    let c8 = v (get h1 c 8) in
-    ( c0 = a0 * b0
-      /\ c1 = a0 * b1 + a1 * b0
-      /\ c2 = a0 * b2 + a1 * b1 + a2 * b0
-      /\ c3 = a0 * b3 + a1 * b2 + a2 * b1 + a3 * b0
-      /\ c4 = a0 * b4 + a1 * b3 + a2 * b2 + a3 * b1 + a4 * b0
-      /\ c5 = a1 * b4 + a2 * b3 + a3 * b2 + a4 * b1
-      /\ c6 = a2 * b4 + a3 * b3 + a4 * b2
-      /\ c7 = a3 * b4 + a4 * b3
-      /\ c8 = a4 * b4 ) )
+(* let isMultiplication (h0:mem) (h1:mem) (a:bigint) (b:bigint) (c:bigint_wide) : GTot Type0 = *)
+(*   live h0 a /\ live h0 b /\ live h1 c *)
+(*   /\ length a >= norm_length /\ length b >= norm_length /\ length c >= 2*norm_length-1 *)
+(*   /\ ( *)
+(*     let a0 = v (get h0 a 0) in let a1 = v (get h0 a 1) in let a2 = v (get h0 a 2) in *)
+(*     let a3 = v (get h0 a 3) in let a4 = v (get h0 a 4) in let b0 = v (get h0 b 0) in *)
+(*     let b1 = v (get h0 b 1) in let b2 = v (get h0 b 2) in let b3 = v (get h0 b 3) in *)
+(*     let b4 = v (get h0 b 4) in *)
+(*     let open Hacl.UInt128 in *)
+(*     let c0 = v (get h1 c 0) in let c1 = v (get h1 c 1) in *)
+(*     let c2 = v (get h1 c 2) in let c3 = v (get h1 c 3) in let c4 = v (get h1 c 4) in *)
+(*     let c5 = v (get h1 c 5) in let c6 = v (get h1 c 6) in let c7 = v (get h1 c 7) in *)
+(*     let c8 = v (get h1 c 8) in *)
+(*     ( c0 = a0 * b0 *)
+(*       /\ c1 = a0 * b1 + a1 * b0 *)
+(*       /\ c2 = a0 * b2 + a1 * b1 + a2 * b0 *)
+(*       /\ c3 = a0 * b3 + a1 * b2 + a2 * b1 + a3 * b0 *)
+(*       /\ c4 = a0 * b4 + a1 * b3 + a2 * b2 + a3 * b1 + a4 * b0 *)
+(*       /\ c5 = a1 * b4 + a2 * b3 + a3 * b2 + a4 * b1 *)
+(*       /\ c6 = a2 * b4 + a3 * b3 + a4 * b2 *)
+(*       /\ c7 = a3 * b4 + a4 * b3 *)
+(*       /\ c8 = a4 * b4 ) ) *)
 
-let isMultiplication_
-  (h1:mem)
-  (a0:int) (a1:int) (a2:int) (a3:int) (a4:int)
-  (b0:int) (b1:int) (b2:int) (b3:int) (b4:int)
-  (c:bigint_wide) : GTot Type0 =
-  live h1 c /\ length c >= 2*norm_length-1
-  /\ (let open Hacl.UInt128 in
-      let c0 = v (get h1 c 0) in let c1 = v (get h1 c 1) in
-      let c2 = v (get h1 c 2) in let c3 = v (get h1 c 3) in let c4 = v (get h1 c 4) in
-      let c5 = v (get h1 c 5) in let c6 = v (get h1 c 6) in let c7 = v (get h1 c 7) in
-      let c8 = v (get h1 c 8) in
-      ( c0 = a0 * b0
-	/\ c1 = a0 * b1 + a1 * b0
-	/\ c2 = a0 * b2 + a1 * b1 + a2 * b0
-	/\ c3 = a0 * b3 + a1 * b2 + a2 * b1 + a3 * b0
-	/\ c4 = a0 * b4 + a1 * b3 + a2 * b2 + a3 * b1 + a4 * b0
-	/\ c5 = a1 * b4 + a2 * b3 + a3 * b2 + a4 * b1
-	/\ c6 = a2 * b4 + a3 * b3 + a4 * b2
-	/\ c7 = a3 * b4 + a4 * b3
-	/\ c8 = a4 * b4 ) )
+(* let isMultiplication_ *)
+(*   (h1:mem) *)
+(*   (a0:int) (a1:int) (a2:int) (a3:int) (a4:int) *)
+(*   (b0:int) (b1:int) (b2:int) (b3:int) (b4:int) *)
+(*   (c:bigint_wide) : GTot Type0 = *)
+(*   live h1 c /\ length c >= 2*norm_length-1 *)
+(*   /\ (let open Hacl.UInt128 in *)
+(*       let c0 = v (get h1 c 0) in let c1 = v (get h1 c 1) in *)
+(*       let c2 = v (get h1 c 2) in let c3 = v (get h1 c 3) in let c4 = v (get h1 c 4) in *)
+(*       let c5 = v (get h1 c 5) in let c6 = v (get h1 c 6) in let c7 = v (get h1 c 7) in *)
+(*       let c8 = v (get h1 c 8) in *)
+(*       ( c0 = a0 * b0 *)
+(* 	/\ c1 = a0 * b1 + a1 * b0 *)
+(* 	/\ c2 = a0 * b2 + a1 * b1 + a2 * b0 *)
+(* 	/\ c3 = a0 * b3 + a1 * b2 + a2 * b1 + a3 * b0 *)
+(* 	/\ c4 = a0 * b4 + a1 * b3 + a2 * b2 + a3 * b1 + a4 * b0 *)
+(* 	/\ c5 = a1 * b4 + a2 * b3 + a3 * b2 + a4 * b1 *)
+(* 	/\ c6 = a2 * b4 + a3 * b3 + a4 * b2 *)
+(* 	/\ c7 = a3 * b4 + a4 * b3 *)
+(* 	/\ c8 = a4 * b4 ) ) *)
 
 private val multiplication_0:
   c:bigint_wide{length c >= 2*norm_length-1} ->
@@ -85,32 +87,34 @@ private val multiplication_0:
     (ensures  (fun h0 _ h1 -> modifies_1 c h0 h1 /\ live h1 c
       /\ isMultiplication_ h1 (v a0) (v a1) (v a2) (v a3) (v a4) (v b0) (v b1) (v b2) (v b3) (v b4) c))
 let multiplication_0 c a0 a1 a2 a3 a4 b0 b1 b2 b3 b4 =
-  (* lemma_multiplication_0 a0 a1 a2 a3 a4 b0 b1 b2 b3 b4; *)
-  let ab00 = a0 *| b0 in
-  let ab01 = a0 *| b1 in
-  let ab02 = a0 *| b2 in
-  let ab03 = a0 *| b3 in
-  let ab04 = a0 *| b4 in
-  let ab10 = a1 *| b0 in
-  let ab11 = a1 *| b1 in
-  let ab12 = a1 *| b2 in
-  let ab13 = a1 *| b3 in
-  let ab14 = a1 *| b4 in
-  let ab20 = a2 *| b0 in
-  let ab21 = a2 *| b1 in
-  let ab22 = a2 *| b2 in
-  let ab23 = a2 *| b3 in
-  let ab24 = a2 *| b4 in
-  let ab30 = a3 *| b0 in
-  let ab31 = a3 *| b1 in
-  let ab32 = a3 *| b2 in
-  let ab33 = a3 *| b3 in
-  let ab34 = a3 *| b4 in
-  let ab40 = a4 *| b0 in
-  let ab41 = a4 *| b1 in
-  let ab42 = a4 *| b2 in
-  let ab43 = a4 *| b3 in
-  let ab44 = a4 *| b4 in
+  lemma_multiplication_0 a0 a1 a2 a3 a4 b0 b1 b2 b3 b4;
+  let open Hacl.UInt128 in
+  let ab00 = a0 *^ b0 in
+  let ab01 = a0 *^ b1 in
+  let ab02 = a0 *^ b2 in
+  let ab03 = a0 *^ b3 in
+  let ab04 = a0 *^ b4 in
+  let ab10 = a1 *^ b0 in
+  let ab11 = a1 *^ b1 in
+  let ab12 = a1 *^ b2 in
+  let ab13 = a1 *^ b3 in
+  let ab14 = a1 *^ b4 in
+  let ab20 = a2 *^ b0 in
+  let ab21 = a2 *^ b1 in
+  let ab22 = a2 *^ b2 in
+  let ab23 = a2 *^ b3 in
+  let ab24 = a2 *^ b4 in
+  let ab30 = a3 *^ b0 in
+  let ab31 = a3 *^ b1 in
+  let ab32 = a3 *^ b2 in
+  let ab33 = a3 *^ b3 in
+  let ab34 = a3 *^ b4 in
+  let ab40 = a4 *^ b0 in
+  let ab41 = a4 *^ b1 in
+  let ab42 = a4 *^ b2 in
+  let ab43 = a4 *^ b3 in
+  let ab44 = a4 *^ b4 in
+  let open Hacl.UInt64 in
   let c0 = ab00 in
   cut (H128.v c0 = v a0 * v b0);
   let c1 = H128 (ab01 +^ ab10) in
@@ -156,181 +160,9 @@ val multiplication:
      (requires (fun h -> norm h a /\ norm h b /\ live h c))
      (ensures (fun h0 u h1 -> norm h0 a /\ norm h0 b /\ live h1 c /\ modifies_1 c h0 h1
        /\ eval_wide h1 c (2*norm_length-1) = eval h0 a (norm_length) * eval h0 b (norm_length)
-       /\ maxValue_wide h1 c (2*norm_length-1) <= norm_length * pow2 53))
+       /\ maxValue_wide h1 c (2*norm_length-1) <= norm_length * pow2 102))
 let multiplication c a b =
   let h0 = ST.get() in
-  multiplication_ c a b(* ; *)
-  (* let h1 = ST.get() in *)
-  (* lemma_multiplication h0 h1 c a b *)
-
-(*
-val multiplication_step_0: a:bigint -> b:bigint ->
-  ctr:u32{U32.v ctr<norm_length /\ U32.v ctr<2*norm_length-1} ->
-  c:bigint_wide{disjoint a c /\ disjoint b c} ->
-  tmp:bigint_wide{disjoint a tmp /\ disjoint b tmp /\ disjoint c tmp} -> Stack unit
-     (requires (fun h -> live h a /\ live h b /\ live h c /\ live h tmp /\ length c >= 2*norm_length-1
-       (* norm h a /\ norm h b /\ live h c /\ live h tmp *)
-       (*  /\ length c >= 2*norm_length -1 *)
-       (* 	/\ maxValueNorm h a < pow2 max_limb *)
-       (* 	/\ maxValueNorm h b < pow2 max_limb *)
-       (* 	/\ maxValue_wide h c (length c) <= w ctr * maxValueNorm h a * maxValueNorm h b *)
-       ))
-     (ensures (fun h0 _ h1 -> live h1 tmp /\ modifies_1 tmp h0 h1
-       (* norm h0 a /\ norm h0 b /\ live h0 c /\ live h1 tmp *)
-       (* /\ live h0 tmp /\ length tmp = length tmp *)
-       (* /\ length c >= 2*norm_length-1 /\ length tmp >= norm_length *)
-       (* /\ modifies_1 tmp h0 h1 *)
-       (* /\ isScalarProduct h1 tmp h0 a (get h0 b (w ctr)) *)
-       (* /\ eval_wide h1 tmp norm_length = eval h0 a norm_length * vv (get h0 b (w ctr)) *)
-     ))
-let multiplication_step_0 a b ctr c tmp =
-  (* admit(); // OK *)
-  (* let h0 = ST.get() in *)
-  let s = b.(ctr) in
-  (* assert(forall (n:nat). {:pattern (vv (get h0 b n))} n < norm_length ==> vv (get h0 b n) <= pow2 max_limb);  *)
-  (* assert(forall (n:nat). n = w ctr ==> n < norm_length);  *)
-  (* assert(True /\ vv s < pow2 max_limb);  *)
-  (* assert(forall (i:nat). {:pattern (vv  (get h0 a i))}  *)
-  (* 	   i < norm_length ==> vv (get h0 a i) < pow2 max_limb); *)
-  (* assert(vv s < pow2 max_limb);  *)
-  (* cut(forall (i:nat). (i < norm_length) ==> vv (get h0 a i) * vv s < pow2 platform_wide);  *)
-  Hacl.EC.Curve25519.Bignum.Fscalar.scalar_multiplication_tr tmp a s 0ul(* ; *)
-  (* let h1 = ST.get() in *)
-  (* cut(True /\ vv s = vv (get h0 b (w ctr)));  *)
-  (* assert(Fscalar.isScalarProduct h0 h1 0 norm_length a s tmp);  *)
-  (* is_scalar_product_lemma h0 h1 a s tmp; *)
-  (* Hacl.EC.Curve25519.Bignum.Fscalar.theorem_scalar_multiplication h0 h1 a s norm_length tmp *)
-
-val multiplication_step_p1:
-  a:bigint -> b:bigint -> ctr:u32{U32.v ctr<norm_length} ->
-  c:bigint_wide{disjoint a c /\ disjoint b c} ->
-  tmp:bigint_wide{disjoint a tmp /\ disjoint b tmp /\ disjoint c tmp} -> Stack unit
-     (requires (fun h -> live h a /\ live h b /\ live h c /\ live h tmp /\ length c >= 2*norm_length-1
-        (* /\ norm h a /\ norm h b /\ live h c /\ live h tmp *)
-        (* /\ length c >= 2*norm_length -1 *)
-	(* /\ maxValueNorm h a < pow2 max_limb *)
-	(* /\ maxValueNorm h b < pow2 max_limb *)
-	(* /\ maxValue_wide h c (length c) <= w ctr * maxValueNorm h a * maxValueNorm h b *)
-	(* /\ eval_wide h c (2*norm_length-1) = eval h a (norm_length) * eval h b (w ctr)  *)
-    ))
-     (ensures (fun h0 u h1 -> live h1 c /\ live h1 tmp /\ modifies_2 c tmp h0 h1
-       (* /\ norm h0 a /\ norm h0 b /\ live h0 c /\ live h0 tmp *)
-       (* /\ norm h1 a /\ norm h1 b /\ live h1 c /\ live h1 tmp *)
-       (* /\ length c >= 2*norm_length -1 *)
-       (* /\ modifies_2 c tmp h0 h1 *)
-       (* /\ maxValue_wide h0 c (length c) <= w ctr * maxValueNorm h0 a * maxValueNorm h0 b *)
-       (* /\ maxValue_wide h1 c (length c) <= (w ctr+1) * (maxValueNorm h0 a * maxValueNorm h0 b) *)
-       (* /\ eval_wide h0 c (2*norm_length-1) = eval h0 a (norm_length) * eval h0 b (w ctr) *)
-       (* /\ (eval_wide h1 c (2*norm_length-1) = eval_wide h0 c (2*norm_length-1) + pow2 (bitweight (templ) (w ctr)) * eval h0 a norm_length * vv (get h0 b (w ctr))) *)
-     ))
-let multiplication_step_p1 a b ctr c tmp =
-  (* admit(); // OK *)
-  (* let h0 = ST.get() in *)
-  multiplication_step_0 a b ctr c tmp;
-  (* let h1 = ST.get() in *)
-  (* multiplication_step_lemma_01 h0 h1 a b (w ctr) c tmp;  *)
-  Hacl.EC.Curve25519.Bignum.FsumWide.fsum_index c ctr tmp 0ul nlength 0ul(* ; *)
-  (* let h2 = ST.get() in  *)
-  (* multiplication_step_lemma_02 h0 h1 h2 a b ctr c tmp *)
-
-(* Code : does 1 step of the multiplication (1 scalar multiplication),
-   and infers the appropriate properties on sizes, values and evaluated
-   values for the resulting bigint *)
-val multiplication_step: a:bigint -> b:bigint -> ctr:u32{U32.v ctr < norm_length} ->
-  c:bigint_wide{disjoint a c /\ disjoint b c} ->
-  tmp:bigint_wide{disjoint a tmp /\ disjoint b tmp /\ disjoint c tmp} -> STL unit
-     (requires (fun h -> live h a /\ live h b /\ live h c /\ live h tmp /\ length c >= 2*norm_length-1
-       (* norm h a /\ norm h b /\ live h c /\ live h tmp *)
-       (* 	/\ length c >= 2 * norm_length - 1 *)
-       (* 	/\ maxValueNorm h a < pow2 max_limb *)
-       (* 	/\ maxValueNorm h b < pow2 max_limb *)
-       (* 	/\ maxValue_wide h c (length c) <= w ctr * maxValueNorm h a * maxValueNorm h b *)
-       (* 	/\ eval_wide h c (2*norm_length-1) = eval h a (norm_length) * eval h b (w ctr) *)
-    ))
-     (ensures (fun h0 u h1 -> live h1 c /\ live h1 tmp /\ modifies_2 c tmp h0 h1
-       (* /\ norm h0 a /\ norm h1 a /\ norm h0 b /\ norm h1 b *)
-       (* /\ live h0 c /\ live h1 c  /\ live h0 tmp /\ live h1 tmp *)
-       (* /\ length c >= 2 * norm_length - 1 *)
-       (* /\ modifies_2 c tmp h0 h1 *)
-       (* /\ maxValueNorm h0 a < pow2 max_limb *)
-       (* /\ maxValueNorm h0 b < pow2 max_limb *)
-       (* /\ maxValue_wide h0 c (length c) <= w ctr * maxValueNorm h0 a * maxValueNorm h0 b *)
-       (* /\ maxValue_wide h1 c (length c) <= (w ctr+1) * maxValueNorm h0 a * maxValueNorm h0 b *)
-       (* /\ eval_wide h0 c (2*norm_length-1) = eval h0 a (norm_length) * eval h0 b (w ctr) *)
-       (* /\ eval_wide h1 c (2*norm_length-1) = eval h0 a (norm_length) * vv (get h0 b (w ctr)) * pow2 (bitweight (templ) (w ctr)) + eval_wide h0 c (2*norm_length-1) *)
-     ))
-let multiplication_step a b ctr c tmp =
-  (* let h0 = ST.get() in *)
-  multiplication_step_p1 a b ctr c tmp(* ;   *)
-  (* let h1 = ST.get() in *)
-  (* helper_lemma_6 h0 h1 a b (w ctr) c tmp *)
-
-(* Code : tail recursive calls to run the multiplication *)
-val multiplication_aux:
-  a:bigint -> b:bigint -> ctr:u32{U32.v ctr <= norm_length} ->
-  c:bigint_wide{disjoint a c /\ disjoint b c} ->
-  tmp:bigint_wide{disjoint a tmp /\ disjoint b tmp /\ disjoint c tmp} -> STL unit
-     (requires (fun h -> live h a /\ live h b /\ live h c /\ live h tmp /\ length c >= 2*norm_length-1
-       (* (norm h a) /\ (norm h b) /\ (live h c) /\ (live h tmp) *)
-       (* 	/\ (length c >= 2 * norm_length - 1) *)
-       (* 	/\ (maxValueNorm h a < pow2 max_limb) *)
-       (* 	/\ (maxValueNorm h b < pow2 max_limb) *)
-       (* 	/\ (maxValue_wide h c (length c) <= (norm_length - w ctr) * (maxValueNorm h a * maxValueNorm h b)) *)
-       (* 	/\ (eval_wide h c (2*norm_length-1) = eval h a (norm_length) * eval h b (norm_length - w ctr)) *)
-    ))
-     (ensures (fun h0 u h1 -> live h1 c /\ live h1 tmp /\ modifies_2 c tmp h0 h1
-       (* (norm h0 a) /\ (norm h0 b) /\ (live h0 c) /\ (live h0 tmp) *)
-       (* /\ (norm h1 a) /\ (norm h1 b) /\ (live h1 c) /\ (live h1 tmp) *)
-       (* /\ (length c >= 2 * norm_length - 1) *)
-       (* /\ (modifies_2 c tmp h0 h1) *)
-       (* /\ (maxValueNorm h0 a < pow2 max_limb) *)
-       (* /\ (maxValueNorm h0 b < pow2 max_limb) *)
-       (* /\ (eval_wide h1 c (2*norm_length-1) = eval h0 a (norm_length) * eval h0 b (norm_length)) *)
-       (* /\ (maxValue_wide h1 c (length c) <= norm_length * (maxValueNorm h0 a * maxValueNorm h0 b)) *)
-     ))
-let rec multiplication_aux a b ctr c tmp =
-  (* let h0 = ST.get() in *)
-  if U32 (ctr =^ 0ul) then ()
-  else begin
-    (* FproductLemmas.helper_lemma_8 norm_length ctr; *)
-    multiplication_step a b (U32 (nlength -^ ctr)) c tmp;
-    (* let h1 = ST.get() in     *)
-    (* multiplication_aux_lemma h0 h1 a b (w ctr) c tmp; *)
-    multiplication_aux a b (U32 (ctr -^ 1ul)) c tmp(* ; *)
-    (* let h2 = ST.get() in *)
-    (* multiplication_aux_lemma_2 h0 h1 h2 a b (w ctr) c tmp *)
-  end
-
-(* Code : core multiplication function *)
-val multiplication:
-  c:bigint_wide ->
-  a:bigint{disjoint c a} ->
-  b:bigint{disjoint c b} -> Stack unit
-    (requires (fun h -> live h c /\ live h a /\ live h b /\ length c >= 2*norm_length-1
-     (* norm h a /\ norm h b /\ live h c /\ null_wide h c /\ length c >= 2*norm_length-1 *)
-     (* 	/\ maxValueNorm h a < pow2 max_limb *)
-     (* 	/\ maxValueNorm h b < pow2 max_limb  *)
-    ))
-    (ensures (fun h0 u h1 -> live h1 c /\ modifies_1 c h0 h1
-      (* /\ norm h0 a /\ norm h0 b /\ live h0 c /\ norm h1 a /\ norm h1 b /\ live h1 c *)
-      (*  /\ length c >= 2*norm_length-1 *)
-      (*  /\ null_wide h0 c /\ modifies_1 c h0 h1 *)
-      (*  /\ maxValueNorm h0 a < pow2 max_limb *)
-      (*  /\ maxValueNorm h0 b < pow2 max_limb *)
-      (*  /\ eval_wide h1 c (2*norm_length-1) = eval h0 a (norm_length) * eval h0 b (norm_length) *)
-      (*  /\ maxValue_wide h1 c (length c) <= norm_length * maxValueNorm h0 a * maxValueNorm h0 b  *)
-    ))
-let multiplication c a b =
-  push_frame();
-  (* admit(); // OK *)
-  (* let h0 = ST.get() in *)
-  let tmp = create (Hacl.Cast.uint64_to_sint128 0uL) nlength in
-  (* let h1 = ST.get() in *)
-  (* assert(modifies Set.empty h0 h1);  *)
-  (* multiplication_lemma_1 h0 h1 c a b; *)
-  (* cut(True /\ length tmp >= norm_length); *)
-  (* constant_template_lemma c a;  *)
-  multiplication_aux a b nlength c tmp;
-  (* let h2 = ST.get() in  *)
-  (* multiplication_lemma_2 h0 h1 h2 c a b tmp *)
-  pop_frame()
+  multiplication_ c a b;
+  let h1 = ST.get() in
+  lemma_multiplication h0 h1 c a b
