crypto/ec/Hacl.EC.Curve25519.Bignum.Fscalar.Lemmas.fst
@@ -44,160 +44,37 @@ let bound115 h (b:bigint_wide) : GTot Type0 =
   /\ v (get h b 4) < pow2 115
 
 
-(*
-#reset-options
+#reset-options "--z3timeout 5 --initial_fuel 0 --max_fuel 0"
 
-(* Lemma *)
-val scalar_multiplication_lemma_aux: h0:heap -> h1:heap -> a:bigint{live h0 a} -> 
-  b:bigint_wide{live h1 b} -> s:int -> len:pos{ (len <= length a)  /\ (len <= length b) } ->
-  Lemma
-    (requires ( (eval h0 a (len-1) * s = eval_wide h1 b (len-1))
-		/\ (v (get h0 a (len-1)) * s = Hacl.UInt128.v (get h1 b (len-1)))))
-    (ensures ( eval h0 a len * s = eval_wide h1 b len ))
-let scalar_multiplication_lemma_aux h0 h1 a b s len =
-//  admit();
-  Math.Axioms.paren_mul_left (pow2 (bitweight (templ) (len-1))) (v (get h0 a (len-1))) s;
-  Math.Axioms.distributivity_add_left ((pow2 (bitweight (templ) (len-1))) * (v (get h0 a (len-1)))) (eval h0 a (len-1)) s
-
-#reset-options
-
-(* Lemma *)
-val scalar_multiplication_lemma: h0:heap -> h1:heap -> a:bigint{live h0 a} -> 
-  b:bigint_wide{live h1 b} -> s:int -> len:nat{len <= length a /\ len <= length b} ->
-  Lemma
-    (requires (forall (i:nat). i < len ==> v (get h0 a i) * s = Hacl.UInt128.v (get h1 b i)))
-    (ensures (eval h0 a len * s = eval_wide h1 b len))
-let rec scalar_multiplication_lemma h0 h1 a b s len =
-//  admit();
-  match len with
-  | 0 -> 
-    assert(eval h0 a len = 0); ()
-    (* FscalarLemmas.lemma_1 s *)
-  | _ -> 
-    (* FscalarLemmas.lemma_3 len; *)
-    scalar_multiplication_lemma h0 h1 a b s (len-1); 
-    scalar_multiplication_lemma_aux h0 h1 a b s len
-
-val scalar_multiplication_tr_1: res:bigint_wide -> a:bigint{disjoint res a} -> s:s64 -> 
-  ctr:u32{w ctr<norm_length} -> STL unit
-     (requires (fun h -> 
-       (live h res) /\ (live h a) /\ (length a >= norm_length) /\ (length res >= norm_length)
-       /\ (forall (i:nat). (i >= w ctr /\ i < norm_length) ==> v (get h a i) * v s < pow2 platform_wide)))
-     (ensures (fun h0 u h1 -> 
-       (live h0 res) /\ (live h1 res) /\ (live h0 a) /\ (live h1 a)
-       /\ (length res >= norm_length) /\ (length res = length res)
-       /\ (modifies_1 res h0 h1) /\ (length a >= norm_length)
-       /\ (forall (i:nat). (i >= w ctr+1 /\ i < norm_length) ==> v (get h0 a i) * v s < pow2 platform_wide) 
-       /\ (forall (i:nat). (i < length res /\ i <> w ctr) ==> (get h1 res i == get h0 res i))
-       /\ (Hacl.UInt128.v (get h1 res (w ctr)) = v (get h0 a (w ctr)) * v s)
-     ))
-let rec scalar_multiplication_tr_1 res a s ctr =
-    let ai = index a ctr in
-    let z = Hacl.UInt128.mul_wide ai s in
-    upd res ctr z
-
-val scalar_multiplication_tr_2:
-  h0:heap -> h1:heap -> h2:heap -> res:bigint_wide -> a:bigint{disjoint res a} -> s:s64 -> ctr:nat{ctr<norm_length} -> 
-  Lemma
-     (requires (
-       (live h1 res) /\ (live h2 res) /\ (live h1 a) /\ (live h2 a) /\ live h0 a /\ live h0 res
-       /\ modifies_1 res h0 h1
-       /\ (modifies_1 res h1 h2) /\ (length a >= norm_length)
-       /\ (forall (i:nat). {:pattern (get h1 a i)} (i >= ctr+1 /\ i < norm_length) ==> v (get h1 a i) * v s < pow2 platform_wide)
-       /\ (length res >= norm_length) /\ (length res = length res)
-       /\ length res = length res
-       /\ (forall (i:nat). {:pattern (get h1 res i)} (i < length res /\ i <> ctr) ==> get h1 res i == get h0 res i)
-       /\ vv (get h1 res ctr) = v (get h0 a ctr) * v s
-       /\ (forall (i:nat{(i>= ctr+1 /\ i < norm_length)}). {:pattern (get h2 res i)} vv (get h2 res i) = v (get h1 a i) * v s)
-       /\ (forall (i:nat{(i < length res /\ (i < ctr+1 \/ i >= norm_length))}). {:pattern (get h2 res i)}
-	   (get h2 res i == get h1 res i))
-       /\ (Seq.equal (sel h1 (a)) (sel h2 (a))) ))
-     (ensures (
-       (live h0 res) /\ (live h2 res) /\ (live h0 a) /\ (live h2 a)
-       /\ (modifies_1 res h0 h2) /\ (length a >= norm_length)
-       /\ (forall (i:nat). (i >= ctr /\ i < norm_length) ==> v (get h0 a i) * v s < pow2 platform_wide)
-       /\ (length res >= norm_length) /\ (length res = length res)
-       /\ (forall (i:nat{(i>= ctr /\ i < norm_length)}). vv (get h2 res i) = v (get h0 a i) * v s)
-       /\ (forall (i:nat{(i < length res /\ (i < ctr \/ i >= norm_length))}). 
-	   (get h2 res i == get h0 res i))
-       /\ (Seq.equal (sel h0 (a)) (sel h2 (a)))
-     ))
-let scalar_multiplication_tr_2 h0 h1 h2 res a s ctr =
-  (* no_upd_lemma h0 h1 a (only res); *)
-  (* no_upd_lemma h1 h2 a (only res); *)
-  ()
-
-(* Code *)
-(* Tail recursive version of the scalar multiplication *)
-val scalar_multiplication_tr: res:bigint_wide -> a:bigint{disjoint res a} -> s:s64 -> ctr:u32{w ctr<=norm_length} -> STL unit
-     (requires (fun h -> 
-       (live h res) /\ (live h a) /\ (length a >= norm_length) /\ (length res >= norm_length)
-       /\ (forall (i:nat). (i >= w ctr /\ i < norm_length) ==> v (get h a i) * v s < pow2 platform_wide)))
-     (ensures (fun h0 u h1 -> 
-       (live h0 res) /\ (live h1 res) /\ (live h0 a) /\ (live h1 a)
-       /\ (modifies_1 res h0 h1) /\ (length a >= norm_length)
-       /\ (forall (i:nat). (i >= w ctr /\ i < norm_length) ==> v (get h0 a i) * v s < pow2 platform_wide)
-       /\ (length res >= norm_length) /\ (length res = length res)
-       /\ (forall (i:nat{(i>= w ctr /\ i < norm_length)}). vv (get h1 res i) = v (get h0 a i) * v s)
-       /\ (forall (i:nat{(i < length res /\ (i < w ctr \/ i >= norm_length))}). 
-	   (get h1 res i == get h0 res i))
-       /\ (Seq.equal (sel h0 (a)) (sel h1 (a)))  ))
-let rec scalar_multiplication_tr res a s ctr =
-  //admit();
-  let h0 = ST.get() in
-  if U32.eq ctr nlength then ()
-  else begin
-     let i = ctr in
-     (* FscalarLemmas.lemma_4 norm_length ctr;  *)
-     scalar_multiplication_tr_1 res a s ctr; 
-     let h1 = ST.get() in 
-     (* no_upd_lemma h0 h1 a (only res); *)
-     scalar_multiplication_tr res a s (ctr+|1ul); 
-     let h2 = ST.get() in
-     scalar_multiplication_tr_2 h0 h1 h2 res a s (w ctr)
-  end
-
-(* Lemma *)   	 
-val theorem_scalar_multiplication: h0:heap -> h1:heap -> a:bigint{live h0 a} -> s:s64 -> 
-  len:nat{len <= length a} -> b:bigint_wide{live h1 b /\ len <= length b} -> Lemma
-    (requires (forall (i:nat). i < len ==> vv (get h1 b i) = v (get h0 a i) * v s))
-    (ensures ((eval_wide h1 b len) = (eval h0 a len) * v s))
-let theorem_scalar_multiplication h0 h1 a s len b = 
-  scalar_multiplication_lemma h0 h1 a b (v s) len; ()
-
-#reset-options
-
-val auxiliary_lemma_2: ha:heap -> a:bigint{norm ha a} -> s:s64 -> i:nat{ i < norm_length} -> Lemma
-    (requires (True))
-    (ensures (v (get ha a i) * v s < pow2 (platform_wide)))
-let auxiliary_lemma_2 ha a s i =
-  (* UInt.mul_lemma #(templ i) (v (get ha a i)) #platform_size (v s); *)
-  Curve.Parameters.parameters_lemma_0 ();
-  (* Math.Lib.pow2_increases_2 platform_wide (templ i + platform_size) *)
-  ()
-  
-val auxiliary_lemma_0: ha:heap -> a:bigint{norm ha a} -> s:s64 -> Lemma
-  (forall (i:nat). i < norm_length ==> v (get ha a i) * v s < pow2 platform_wide)
-let auxiliary_lemma_0 ha a s = ()
-
-val auxiliary_lemma_1: h0:heap -> h1:heap -> b:bigint{norm h0 b} -> #t:Type -> b':buffer t ->
-  Lemma (requires (live h1 b /\ modifies_1 b' h0 h1 /\ disjoint b b'))
-	(ensures (norm h1 b))
-let auxiliary_lemma_1 h0 h1 b #t b' = ()
-
-val scalar': res:bigint_wide -> a:bigint{disjoint res a} -> s:s64 -> STL unit
-     (requires (fun h -> norm h a /\ live h res))
-     (ensures (fun h0 u h1 -> live h0 res /\ live h1 res /\ norm h0 a /\ norm h1 a
-       /\ modifies_1 res h0 h1
-       /\ eval_wide h1 res norm_length = eval h0 a norm_length * v s ))
-let scalar' res a s =
-  let h0 = ST.get() in  
-  auxiliary_lemma_0 h0 a s; 
-  scalar_multiplication_tr res a s 0ul; 
-  let h1 = ST.get() in
-  (* no_upd_lemma h0 h1 a (only res); *)
-  auxiliary_lemma_1 h0 h1 a (res); 
-  theorem_scalar_multiplication h0 h1 a s norm_length res; 
-  ()
-
-	       
+val lemma_fscalar:
+  h0:mem -> h1:mem ->
+  res:bigint_wide ->
+  a:bigint ->
+  s:s64 ->
+  Lemma (requires (isScalarMult h0 h1 res a s /\ norm h0 a))
+        (ensures  (isScalarMult h0 h1 res a s /\ norm h0 a
+          /\ bound115 h1 res
+          /\ eval_wide h1 res norm_length = eval h0 a norm_length * v s))
+let lemma_fscalar h0 h1 res a s =
+  assert_norm(pow2 115 = 41538374868278621028243970633760768);
+  assert_norm(pow2 64 = 18446744073709551616);
+  assert_norm(pow2 51 = 2251799813685248);
+  Math.Lemmas.lemma_mult_le_right (v s) (v (get h0 a 0)) (pow2 51 - 1);
+  Math.Lemmas.lemma_mult_le_right (v s) (v (get h0 a 1)) (pow2 51 - 1);
+  Math.Lemmas.lemma_mult_le_right (v s) (v (get h0 a 2)) (pow2 51 - 1);
+  Math.Lemmas.lemma_mult_le_right (v s) (v (get h0 a 3)) (pow2 51 - 1);
+  Math.Lemmas.lemma_mult_le_right (v s) (v (get h0 a 4)) (pow2 51 - 1);
+  lemma_eval_bigint_5 h0 a;
+  lemma_eval_bigint_wide_5 h1 res;
+  cut (eval_wide h1 res norm_length =
+    (v (get h0 a 0) * v s) + pow2 51 * (v (get h0 a 1) * v s) + pow2 102 * (v (get h0 a 2) * v s) +
+      pow2 153 * (v (get h0 a 3) * v s) + pow2 204 * (v (get h0 a 4) * v s));
+  Math.Lemmas.paren_mul_right (pow2 51) (v (get h0 a 1)) (v s);
+  Math.Lemmas.paren_mul_right (pow2 102) (v (get h0 a 2)) (v s);
+  Math.Lemmas.paren_mul_right (pow2 153) (v (get h0 a 3)) (v s);
+  Math.Lemmas.paren_mul_right (pow2 204) (v (get h0 a 4)) (v s);
+  Math.Lemmas.distributivity_add_left (v (get h0 a 0)) (pow2 51 * v (get h0 a 1)) (v s);
+  Math.Lemmas.distributivity_add_left (v (get h0 a 0) + pow2 51 * v (get h0 a 1))
+                                      (pow2 102 * v (get h0 a 2)) (v s);
+  Math.Lemmas.distributivity_add_left (v (get h0 a 0) + pow2 51 * v (get h0 a 1) + pow2 102 * v (get h0 a 2)) (pow2 153 * v (get h0 a 3)) (v s);
+  Math.Lemmas.distributivity_add_left (v (get h0 a 0) + pow2 51 * v (get h0 a 1) + pow2 102 * v (get h0 a 2) + pow2 153 * v (get h0 a 3)) (pow2 204 * v (get h0 a 4)) (v s)
