crypto/ec/Hacl.EC.Curve25519.Bignum.Fscalar.fst
@@ -33,7 +33,7 @@ val fscalar_:
   a:bigint{disjoint res a} ->
   s:s64 ->
   Stack unit
-    (requires (fun h -> norm h a))
+    (requires (fun h -> live h res /\ norm h a))
     (ensures (fun h0 _ h1 -> live h1 res /\ modifies_1 res h0 h1 /\ isScalarMult h0 h1 res a s))
 let fscalar_ res a s =
   Math.Lemmas.pow2_lt_compat 64 51; Math.Lemmas.pow2_plus 51 64; Math.Lemmas.pow2_plus 64 64;
@@ -48,76 +48,18 @@ let fscalar_ res a s =
   let r2 = a2 *^ s in
   let r3 = a3 *^ s in
   let r4 = a4 *^ s in
-  update_5 res r0 r1 r2 r3 r4
+  update_wide_5 res r0 r1 r2 r3 r4
 
-(*
-
-
-val scalar_multiplication_tr_1: 
-  res:bigint_wide -> a:bigint{disjoint res a} -> s:s64 -> 
-  ctr:u32{U32.v ctr<norm_length} -> Stack unit
-     (requires (fun h -> live h a /\ live h res
-       (* (live h res) /\ (live h a) /\ (length a >= norm_length) /\ (length res >= norm_length) *)
-       (* /\ (forall (i:nat). (i >= w ctr /\ i < norm_length) ==> v (get h a i) * v s < pow2 platform_wide) *)
-     ))
-     (ensures (fun h0 u h1 -> live h1 res /\ modifies_1 res h0 h1
-       (* (live h0 res) /\ (live h1 res) /\ (live h0 a) /\ (live h1 a) *)
-       (* /\ (length res >= norm_length) /\ (length res = length res) *)
-       (* /\ (modifies_1 res h0 h1) /\ (length a >= norm_length) *)
-       (* /\ (forall (i:nat). (i >= w ctr+1 /\ i < norm_length) ==> v (get h0 a i) * v s < pow2 platform_wide)  *)
-       (* /\ (forall (i:nat). (i < length res /\ i <> w ctr) ==> (get h1 res i == get h0 res i)) *)
-       (* /\ (Hacl.UInt128.v (get h1 res (w ctr)) = v (get h0 a (w ctr)) * v s) *)
-     ))
-let rec scalar_multiplication_tr_1 res a s ctr =
-    let ai = a.(ctr) in
-    let z = Hacl.UInt128.mul_wide ai s in
-    res.(ctr) <- z
-
-val scalar_multiplication_tr: res:bigint_wide -> a:bigint{disjoint res a} -> s:s64 -> ctr:u32{U32.v ctr<=norm_length} -> Stack unit
-     (requires (fun h -> live h res /\ live h a
-       (* (live h res) /\ (live h a) /\ (length a >= norm_length) /\ (length res >= norm_length) *)
-       (* /\ (forall (i:nat). (i >= w ctr /\ i < norm_length) ==> v (get h a i) * v s < pow2 platform_wide) *)
-     ))
-     (ensures (fun h0 u h1 -> live h1 res /\ modifies_1 res h0 h1
-       (* (live h0 res) /\ (live h1 res) /\ (live h0 a) /\ (live h1 a) *)
-       (* /\ (modifies_1 res h0 h1) /\ (length a >= norm_length) *)
-       (* /\ (forall (i:nat). (i >= w ctr /\ i < norm_length) ==> v (get h0 a i) * v s < pow2 platform_wide) *)
-       (* /\ (length res >= norm_length) /\ (length res = length res) *)
-       (* /\ (forall (i:nat{(i>= w ctr /\ i < norm_length)}). vv (get h1 res i) = v (get h0 a i) * v s) *)
-       (* /\ (forall (i:nat{(i < length res /\ (i < w ctr \/ i >= norm_length))}).  *)
-       (* 	   (get h1 res i == get h0 res i)) *)
-       (* /\ (Seq.equal (sel h0 (a)) (sel h1 (a))) *)
-     ))
-let rec scalar_multiplication_tr res a s ctr =
-  (* let h0 = ST.get() in *)
-  if U32 (ctr =^ nlength) then ()
-  else begin
-     (* FscalarLemmas.lemma_4 norm_length ctr;  *)
-     scalar_multiplication_tr_1 res a s ctr; 
-     (* let h1 = ST.get() in  *)
-     (* no_upd_lemma h0 h1 a (only res); *)
-     scalar_multiplication_tr res a s (U32 (ctr +^ 1ul))
-     (* let h2 = ST.get() in *)
-     (* scalar_multiplication_tr_2 h0 h1 h2 res a s (w ctr) *)
-  end
 
 val scalar': res:bigint_wide -> a:bigint{disjoint res a} -> s:s64 -> STL unit
-     (requires (fun h -> live h a /\ live h res
-       (* norm h a /\ live h res *)
-     ))
-     (ensures (fun h0 u h1 -> live h1 res /\ modifies_1 res h0 h1
-       (* /\ live h0 res /\ live h1 res /\ norm h0 a /\ norm h1 a *)
-       (* /\ modifies_1 res h0 h1 *)
-       (* /\ eval_wide h1 res norm_length = eval h0 a norm_length * v s *)
-     ))
+     (requires (fun h -> norm h a /\ live h res))
+     (ensures (fun h0 u h1 ->
+       live h0 res /\ live h1 res /\ norm h0 a /\ norm h1 a
+       /\ modifies_1 res h0 h1
+       /\ bound115 h1 res
+       /\ eval_wide h1 res norm_length = eval h0 a norm_length * v s ))
 let scalar' res a s =
-  (* let h0 = ST.get() in   *)
-  (* auxiliary_lemma_0 h0 a s;  *)
-  scalar_multiplication_tr res a s 0ul
-  (* let h1 = ST.get() in *)
-  (* (\* no_upd_lemma h0 h1 a (only res); *\) *)
-  (* auxiliary_lemma_1 h0 h1 a (res);  *)
-  (* theorem_scalar_multiplication h0 h1 a s norm_length res;  *)
-  (* () *)
-
-	       
+  let h0 = ST.get() in
+  fscalar_ res a s;
+  let h1 = ST.get() in
+  lemma_fscalar h0 h1 res a s
